verify/CTL.v
@@ -1,0 +1,2616 @@
+From BusyCoq Require Import DHTM.
+Require Import List.
+Require Import Streams.
+Require Import ZArith.
+Require Import Lia.
+From BusyCoq Require Import HashTable.
+Require Uint63.
+
+Module Type CTLCtx(K:HashableType)(Ctx:Ctx).
+Export K.
+Export Ctx.
+Parameter config_t:Type.
+Parameter global_state_t:Type.
+Parameter global_state_init:config_t->global_state_t.
+Parameter dfa_state_0:K.
+Parameter dfa_trans:K->Sym->dir->global_state_t->(K*global_state_t).
+End CTLCtx.
+
+
+Definition int0 := Eval compute in (Uint63.of_Z Z0).
+Definition int1 := Eval compute in (Uint63.of_Z (1%Z)).
+
+Module CTL(K:HashableType)(Ctx:Ctx)(CTLCtx:CTLCtx K Ctx).
+
+Module TM := DHTM Ctx. Export TM.
+Export Ctx.
+Export CTLCtx.
+
+Module IdAllocK := IdAlloc K.
+
+Module QHash := QHash Ctx.
+
+Module SymHash := SymHash Ctx.
+
+Module dfa_trans_V <: ValueType.
+Definition V:Type := Uint63.int*Sym.
+End dfa_trans_V.
+Module dfa_trans_Hash := ProdHash Uint63_K SymHash.
+Module dfa_trans_HashMap := HashMap dfa_trans_Hash Uint63_V.
+Module dfa_trans_inv1_HashMap := HashMultimap dfa_trans_Hash Uint63_V.
+Module dfa_trans_inv2_HashMap := HashMultimap Uint63_K dfa_trans_V.
+
+Module DirHash <: HashableType.
+Import HashConcat.
+Definition K := dir.
+Definition K_hash := fun x =>
+match x with
+| L => hv1
+| R => hv2
+end.
+Definition K_eq a b :=
+match a,b with
+| L,L | R,R => true
+| _,_ => false
+end.
+Lemma K_eq_spec a b: Bool.reflect (a=b) (K_eq a b).
+Proof.
+  destruct a,b; solve_Bool_reflect.
+Qed.
+End DirHash.
+
+Module Unit_V <: ValueType.
+Definition V := unit.
+End Unit_V.
+
+Record config := {
+  l:Uint63.int;
+  r:Uint63.int;
+  s: Q;
+  sgn: dir;
+}.
+
+Module config_Hash <: HashableType.
+Import HashConcat.
+Definition K := config.
+Definition K_hash(a:K) :=
+let (a0,a1,a2,a3):=a in
+(a0 # a1,hash_P) ## (QHash.K_hash a2) ## (DirHash.K_hash a3).
+Definition K_eq(a b:K) :=
+let (a0,a1,a2,a3):=a in
+let (b0,b1,b2,b3):=b in
+(Uint63.eqb a0 b0) &&
+(Uint63.eqb a1 b1) &&
+(q_eqb a2 b2) &&
+(DirHash.K_eq a3 b3).
+Lemma K_eq_spec(a b:K):Bool.reflect (a=b) (K_eq a b).
+Proof.
+  destruct a as [a0 a1 a2 a3].
+  destruct b as [b0 b1 b2 b3].
+  cbn.
+  destruct (Uint63_K.K_eq_spec a0 b0); solve_Bool_reflect.
+  destruct (Uint63_K.K_eq_spec a1 b1); solve_Bool_reflect.
+  destruct (q_eqb_spec a2 b2); solve_Bool_reflect.
+  destruct (DirHash.K_eq_spec a3 b3); solve_Bool_reflect.
+Qed.
+End config_Hash.
+
+Module config_HashSet := HashMap config_Hash Unit_V.
+
+Module config_V <: ValueType.
+Definition V := config.
+End config_V.
+
+Module config_Index := HashMultimap Uint63_K config_V.
+
+Record dfa_t := {
+  id_alloc: IdAllocK.id_alloc_t;
+  trans: dfa_trans_HashMap.hmap_t;
+  inv1_trans: dfa_trans_inv1_HashMap.hmap_t;
+  inv2_trans: dfa_trans_inv2_HashMap.hmap_t;
+  config_idx: config_Index.hmap_t;
+}.
+
+Record CTL_state_t := {
+  ldfa: dfa_t;
+  rdfa: dfa_t;
+  config_set: config_HashSet.hmap_t;
+  config_queue: list (Uint63.int*Sym*(Sym*dir*Q)*config);
+  global_state: global_state_t;
+  init_flag: bool;
+}.
+
+Inductive dfa_match(dfa:dfa_trans_HashMap.hmap_t): list Sym -> Uint63.int -> Prop :=
+| dfa_match_O: dfa_match dfa [] int0
+| dfa_match_S a ls x x':
+  dfa_match dfa ls x ->
+  dfa_trans_HashMap.hmap_get (x,a) dfa = Some x' ->
+  dfa_match dfa (a::ls) x'
+.
+
+Inductive is_config(st:CTL_state_t): DH_config -> config -> Prop :=
+| is_config_l l r l' r' s
+  (Hlm: dfa_match st.(ldfa).(trans) l l')
+  (Hrm: dfa_match st.(rdfa).(trans) r r'):
+  is_config st (const s0 <* r, l *> const s0, s, L) {| l:=r'; r:=l'; s:=s; sgn:=L |}
+| is_config_r l r l' r' s
+  (Hlm: dfa_match st.(ldfa).(trans) l l')
+  (Hrm: dfa_match st.(rdfa).(trans) r r'):
+  is_config st (const s0 <* l, r *> const s0, s, R) {| l:=l'; r:=r'; s:=s; sgn:=R |}
+.
+
+Inductive is_config_in_mset(st:CTL_state_t): DH_config -> config -> Prop :=
+| is_config'_intro c1 c1'
+  (H_is_config: is_config st c1 c1')
+  (H_in_mset: config_HashSet.hmap_get c1' st.(config_set) = Some tt):
+  is_config_in_mset st c1 c1'
+.
+
+Section tm_ctx.
+Hypothesis tm:TM.
+Hypothesis DH_config_init:DH_cconfig.
+
+Definition config_init:DH_config :=
+DH_cconfig_to_config DH_config_init.
+
+Inductive dfa_WF: dfa_t -> CTL_state_t -> dir -> Prop :=
+| dfa_WF_intro dfa st dir
+
+  (H_id_alloc_wf: IdAllocK.id_alloc_WF dfa.(id_alloc))
+  (H_trans_wf: dfa_trans_HashMap.hmap_WF dfa.(trans))
+  (H_inv1_trans_wf: dfa_trans_inv1_HashMap.hmap_WF dfa.(inv1_trans))
+  (H_inv2_trans_wf: dfa_trans_inv2_HashMap.hmap_WF dfa.(inv2_trans))
+  (H_config_idx_wf: config_Index.hmap_WF dfa.(config_idx))
+
+  (H_dfa_state0: dfa_trans_HashMap.hmap_get (int0,s0) dfa.(trans) = Some int0)
+  (H_inv1_trans:
+    forall x y z,
+    dfa_trans_HashMap.hmap_get (x,y) dfa.(trans) = Some z ->
+    In x (dfa_trans_inv1_HashMap.hmap_get (z,y) dfa.(inv1_trans)))
+  (H_inv2_trans:
+    forall x y z,
+    dfa_trans_HashMap.hmap_get (x,y) dfa.(trans) = Some z ->
+    In (x,y) (dfa_trans_inv2_HashMap.hmap_get z dfa.(inv2_trans)))
+  (H_config_idx:
+    forall c,
+    config_HashSet.hmap_get c st.(config_set) = Some tt ->
+    c.(sgn) = dir ->
+    In c (config_Index.hmap_get c.(r) dfa.(config_idx))):
+  dfa_WF dfa st dir
+.
+
+Definition get_dfa(st:CTL_state_t)(sgn:dir) :=
+match sgn with
+| L => st.(ldfa)
+| R => st.(rdfa)
+end.
+
+Definition next_config(cfg:(Uint63.int * Sym * (Sym * dir * Q) * config))(st:CTL_state_t):option config :=
+let '(x,y,y',c1'):=cfg in
+let (l0,r0,s0,sgn0):=c1' in
+let '(y1,sgn1,s1):=y' in
+if DirHash.K_eq sgn0 sgn1 then
+  dfa_trans_HashMap.hmap_get (l0,y1) (get_dfa st (dir_rev sgn0)).(trans) &&& (fun l1 =>
+    Some {| l:=l1; r:=x; s:=s1; sgn:=sgn1 |})
+else
+  dfa_trans_HashMap.hmap_get (x,y1) (get_dfa st sgn0).(trans) &&& (fun r1 =>
+    Some {| l:=r1; r:=l0; s:=s1; sgn:=sgn1 |})
+.
+
+Inductive CTL_state_WF: CTL_state_t -> Prop :=
+| CTL_state_WF_intro st
+  (HO: st.(init_flag) = false \/
+    exists c1',
+    (is_config_in_mset st config_init c1'))
+  (HS: forall c1',
+    config_HashSet.hmap_get c1' st.(config_set) = Some tt ->
+    (forall x y,
+      let (l0,r0,s0,sgn0):=c1' in
+      dfa_trans_HashMap.hmap_get (x,y) (get_dfa st sgn0).(trans) = Some r0 ->
+      exists y',
+      tm (s0,y) = Some y' /\
+      (In (x,y,y',c1') st.(config_queue) \/
+      (exists c2', next_config (x,y,y',c1') st = Some c2' /\ config_HashSet.hmap_get c2' st.(config_set) = Some tt)
+      )))
+  (HL: dfa_WF st.(ldfa) st L)
+  (HR: dfa_WF st.(rdfa) st R)
+  (H_config_set_wf: config_HashSet.hmap_WF st.(config_set)):
+  CTL_state_WF st
+.
+
+Definition get_cs' (x:Uint63.int) (y:Sym) cs :=
+List.fold_right (fun c cs0 => cs0 &&& (fun cs1 => tm (c.(s),y) &&& (fun y' => Some ((x,y,y',c)::cs1)))) (Some nil) cs.
+
+Definition dfa_add_trans(st:CTL_state_t)(x:Uint63.int)(y:Sym)(sgn:dir):option CTL_state_t :=
+let dfa := get_dfa st sgn in
+IdAllocK.get_key x dfa.(id_alloc) &&& (fun x' =>
+let (z',gs) := dfa_trans x' y sgn st.(global_state) in
+IdAllocK.get_or_alloc_id z' dfa.(id_alloc) &&& (fun '(z,id_alloc') =>
+let trans' := dfa_trans_HashMap.hmap_set (x,y) z dfa.(trans) in
+let inv1_trans' := dfa_trans_inv1_HashMap.hmap_add (z,y) x dfa.(inv1_trans) in
+let inv2_trans' := dfa_trans_inv2_HashMap.hmap_add z (x,y) dfa.(inv2_trans) in
+let cs := config_Index.hmap_get z dfa.(config_idx) in
+get_cs' x y cs &&& (fun cs' =>
+let dfa' := {| id_alloc := id_alloc'; trans := trans'; inv1_trans := inv1_trans'; inv2_trans := inv2_trans'; config_idx := dfa.(config_idx) |} in
+Some {|
+  ldfa :=
+  match sgn with
+  | L => dfa'
+  | R => st.(ldfa)
+  end;
+  rdfa :=
+  match sgn with
+  | L => st.(rdfa)
+  | R => dfa'
+  end;
+  config_set := st.(config_set);
+  config_queue := cs' ++ st.(config_queue);
+  global_state := gs;
+  init_flag := st.(init_flag);
+|}
+))).
+
+Definition dfa_add_config(dfa:dfa_t)(sgn0:dir)(c1':config):dfa_t :=
+if DirHash.K_eq c1'.(sgn) sgn0 then
+{|
+  id_alloc := dfa.(id_alloc);
+  trans := dfa.(trans);
+  inv1_trans := dfa.(inv1_trans);
+  inv2_trans := dfa.(inv2_trans);
+  config_idx := config_Index.hmap_add c1'.(r) c1' dfa.(config_idx)
+|}
+else dfa.
+
+Definition get_cs'' c1' (xys:list (Uint63.int*Sym)) :=
+  List.fold_right (fun '(x,y) cs0 => cs0 &&& (fun cs1 => tm (c1'.(s),y) &&& (fun y' => Some ((x,y,y',c1')::cs1)))) (Some nil) xys.
+
+Definition config_push(st:CTL_state_t)(c1':config):option CTL_state_t :=
+match config_HashSet.hmap_add c1' tt st.(config_set) with
+| None =>
+  Some {|
+    ldfa := st.(ldfa);
+    rdfa := st.(rdfa);
+    config_set := st.(config_set);
+    config_queue := List.tl st.(config_queue);
+    global_state := st.(global_state);
+    init_flag := st.(init_flag);
+  |}
+| Some config_set' =>
+  let dfa := get_dfa st c1'.(sgn) in
+  let xys := dfa_trans_inv2_HashMap.hmap_get c1'.(r) dfa.(inv2_trans) in
+  get_cs'' c1' xys &&& (fun cs' =>
+  Some {|
+    ldfa := dfa_add_config st.(ldfa) L c1';
+    rdfa := dfa_add_config st.(rdfa) R c1';
+    config_set := config_set';
+    config_queue := cs' ++ List.tl st.(config_queue);
+    global_state := st.(global_state);
+   init_flag := st.(init_flag);
+  |})
+end.
+
+Definition CTL_step(st:CTL_state_t):option CTL_state_t :=
+match st.(config_queue) with
+| (x,y,y',c1')::q0 =>
+  let (l0,r0,s0,sgn0):=c1' in
+  let '(y1,sgn1,s1):=y' in
+  if DirHash.K_eq sgn0 sgn1 then
+    match dfa_trans_HashMap.hmap_get (l0,y1) (get_dfa st (dir_rev sgn0)).(trans) with
+    | Some l1 => (config_push st {| l:=l1; r:=x; s:=s1; sgn:=sgn1 |})
+    | None => dfa_add_trans st l0 y1 (dir_rev sgn0)
+    end
+  else
+    match dfa_trans_HashMap.hmap_get (x,y1) (get_dfa st sgn0).(trans) with
+    | Some r1 => (config_push st {| l:=r1; r:=l0; s:=s1; sgn:=sgn1 |})
+    | None => dfa_add_trans st x y1 sgn0
+    end
+| _ => None
+end.
+
+Definition dfa_0 len := 
+IdAllocK.get_or_alloc_id dfa_state_0 (IdAllocK.id_alloc_make len) &&& (fun '(z0,id_alloc') =>
+Some {|
+  id_alloc := id_alloc';
+  trans := dfa_trans_HashMap.hmap_set (z0,s0) z0 (dfa_trans_HashMap.hmap_make len);
+  inv1_trans := dfa_trans_inv1_HashMap.hmap_add (z0,s0) z0 (dfa_trans_inv1_HashMap.hmap_make len);
+  inv2_trans := dfa_trans_inv2_HashMap.hmap_add z0 (z0,s0) (dfa_trans_inv2_HashMap.hmap_make len);
+  config_idx := config_Index.hmap_make len;
+|}).
+
+Definition CTL_state_0 cfg len :=
+dfa_0 len &&& (fun dfa0 =>
+Some {|
+  ldfa := dfa0;
+  rdfa := dfa0;
+  config_set := config_HashSet.hmap_make len;
+  config_queue := nil;
+  global_state := global_state_init cfg;
+  init_flag := false;
+|}).
+
+Definition dfa_get_trans st x y sgn0 :=
+  dfa_trans_HashMap.hmap_get (x,y) (get_dfa st sgn0).(trans).
+
+Definition CTL_add_side st sgn0 ls :=
+List.fold_right (fun y st => st &&& (fun '(st,x) => 
+  match dfa_get_trans st x y sgn0 with
+  | Some z => Some (st,z)
+  | None => dfa_add_trans st x y sgn0 &&&
+    (fun st => dfa_get_trans st x y sgn0 &&& (fun z => Some (st,z)))
+  end
+)) (Some (st,int0)) ls.
+
+Definition CTL_state_1 cfg len :=
+let '(l0,r0,s2,sgn0):=DH_config_init in
+CTL_state_0 cfg len &&& (fun st =>
+CTL_add_side st (dir_rev sgn0) l0 &&& (fun '(st,_) =>
+CTL_add_side st sgn0 r0 &&& (fun '(st,_) =>
+Some st
+))).
+
+Definition CTL_match_side st sgn0 ls :=
+List.fold_right (fun y x => x &&& (fun x => 
+  dfa_get_trans st x y sgn0
+)) (Some (int0)) ls.
+
+Definition CTL_state_init cfg len :=
+let '(l0,r0,s2,sgn0):=DH_config_init in
+CTL_state_1 cfg len &&& (fun st =>
+CTL_match_side st (dir_rev sgn0) l0 &&& (fun l1 =>
+CTL_match_side st sgn0 r0 &&& (fun r1 =>
+  let c1' := {| l:=l1; r:=r1; s:=s2; sgn:=sgn0 |} in
+  let config_set' := config_HashSet.hmap_set c1' tt st.(config_set) in
+  let dfa := get_dfa st c1'.(sgn) in
+  let xys := dfa_trans_inv2_HashMap.hmap_get c1'.(r) dfa.(inv2_trans) in
+  get_cs'' c1' xys &&& (fun cs' =>
+  Some {|
+    ldfa := dfa_add_config st.(ldfa) L c1';
+    rdfa := dfa_add_config st.(rdfa) R c1';
+    config_set := config_set';
+    config_queue := cs' ++ st.(config_queue);
+    global_state := st.(global_state);
+    init_flag := true;
+  |})
+))).
+
+Definition CTL_steps cfg len n :=
+N_iter_until (fun st =>
+match CTL_step st with
+| Some st' => inl st'
+| None => inr (Some st)
+end)
+(match CTL_state_init cfg len with
+| Some st => inl st
+| None => inr None
+end) n.
+
+Definition CTL_decide_nonhalt cfg len T :=
+match CTL_steps cfg len T with
+| inr (Some st) =>
+  st.(init_flag) &&
+  match st.(config_queue) with
+  | nil => true
+  | _ => false
+  end
+| _ => false
+end.
+
+
+
+
+Ltac cbn_proj :=
+  cbn[ldfa]; cbn[rdfa]; cbn[config_set]; cbn[config_queue]; cbn[global_state]; cbn[init_flag];
+  cbn[id_alloc]; cbn[config_idx]; cbn[trans]; cbn[inv1_trans]; cbn[inv2_trans].
+
+Lemma CTL_state_0_WF cfg len:
+  match CTL_state_0 cfg len with
+  | Some st => CTL_state_WF st
+  | None => True
+  end.
+Proof.
+  unfold CTL_state_0,dfa_0.
+  unfold dfa_add_trans,if_Some.
+  destruct (IdAllocK.get_or_alloc_id dfa_state_0 (IdAllocK.id_alloc_make len)) as [[z id_alloc']|] eqn:E1; trivial.
+  assert (z=int0). {
+    unfold IdAllocK.get_or_alloc_id,IdAllocK.id_alloc_make in E1.
+    rewrite IdAllocK.MapToId.hmap_get_make in E1.
+    inverts E1.
+    reflexivity.
+  }
+  subst z.
+  constructor;
+  cbn[get_dfa]; cbn_proj.
+  - left. reflexivity.
+  - intros c H.
+    rewrite config_HashSet.hmap_get_make in H. congruence.
+  - constructor; cbn_proj.
+    + epose proof (IdAllocK.get_or_alloc_id_WF _ _ _) as H.
+      rewrite E1 in H.
+      apply H.
+      Unshelve.
+      apply IdAllocK.id_alloc_make_WF.
+    + apply dfa_trans_HashMap.hmap_set_WF,dfa_trans_HashMap.hmap_make_WF.
+    + apply dfa_trans_inv1_HashMap.hmap_add_WF,dfa_trans_inv1_HashMap.hmap_make_WF.
+    + apply dfa_trans_inv2_HashMap.hmap_add_WF,dfa_trans_inv2_HashMap.hmap_make_WF. 
+    + apply config_Index.hmap_make_WF.
+    + apply dfa_trans_HashMap.hmap_get_set_same,dfa_trans_HashMap.hmap_make_WF.
+    + intros x y z E.
+      destruct (dfa_trans_Hash.K_eq_spec (x,y) (int0,s0)).
+      * inverts e.
+        rewrite dfa_trans_HashMap.hmap_get_set_same in E.
+        2: apply dfa_trans_HashMap.hmap_make_WF.
+        inverts E.
+        rewrite dfa_trans_inv1_HashMap.hmap_get_add_same.
+        2: apply dfa_trans_inv1_HashMap.hmap_make_WF.
+        left; reflexivity.
+      * rewrite dfa_trans_HashMap.hmap_get_set_other in E; auto 1.
+        2: apply dfa_trans_HashMap.hmap_make_WF.
+        rewrite dfa_trans_HashMap.hmap_get_make in E; congruence.
+    + intros x y z E.
+      destruct (dfa_trans_Hash.K_eq_spec (x,y) (int0,s0)).
+      * inverts e.
+        rewrite dfa_trans_HashMap.hmap_get_set_same in E.
+        2: apply dfa_trans_HashMap.hmap_make_WF.
+        inverts E.
+        rewrite dfa_trans_inv2_HashMap.hmap_get_add_same.
+        2: apply dfa_trans_inv2_HashMap.hmap_make_WF.
+        left; reflexivity.
+      * rewrite dfa_trans_HashMap.hmap_get_set_other in E; auto 1.
+        2: apply dfa_trans_HashMap.hmap_make_WF.
+        rewrite dfa_trans_HashMap.hmap_get_make in E; congruence.
+    + intros c Hc Hs.
+      rewrite config_HashSet.hmap_get_make in Hc. congruence.
+  - constructor; cbn_proj.
+    + epose proof (IdAllocK.get_or_alloc_id_WF _ _ _) as H.
+      rewrite E1 in H.
+      apply H.
+      Unshelve.
+      apply IdAllocK.id_alloc_make_WF.
+    + apply dfa_trans_HashMap.hmap_set_WF,dfa_trans_HashMap.hmap_make_WF.
+    + apply dfa_trans_inv1_HashMap.hmap_add_WF,dfa_trans_inv1_HashMap.hmap_make_WF.
+    + apply dfa_trans_inv2_HashMap.hmap_add_WF,dfa_trans_inv2_HashMap.hmap_make_WF. 
+    + apply config_Index.hmap_make_WF.
+    + apply dfa_trans_HashMap.hmap_get_set_same,dfa_trans_HashMap.hmap_make_WF.
+    + intros x y z E.
+      destruct (dfa_trans_Hash.K_eq_spec (x,y) (int0,s0)).
+      * inverts e.
+        rewrite dfa_trans_HashMap.hmap_get_set_same in E.
+        2: apply dfa_trans_HashMap.hmap_make_WF.
+        inverts E.
+        rewrite dfa_trans_inv1_HashMap.hmap_get_add_same.
+        2: apply dfa_trans_inv1_HashMap.hmap_make_WF.
+        left; reflexivity.
+      * rewrite dfa_trans_HashMap.hmap_get_set_other in E; auto 1.
+        2: apply dfa_trans_HashMap.hmap_make_WF.
+        rewrite dfa_trans_HashMap.hmap_get_make in E; congruence.
+    + intros x y z E.
+      destruct (dfa_trans_Hash.K_eq_spec (x,y) (int0,s0)).
+      * inverts e.
+        rewrite dfa_trans_HashMap.hmap_get_set_same in E.
+        2: apply dfa_trans_HashMap.hmap_make_WF.
+        inverts E.
+        rewrite dfa_trans_inv2_HashMap.hmap_get_add_same.
+        2: apply dfa_trans_inv2_HashMap.hmap_make_WF.
+        left; reflexivity.
+      * rewrite dfa_trans_HashMap.hmap_get_set_other in E; auto 1.
+        2: apply dfa_trans_HashMap.hmap_make_WF.
+        rewrite dfa_trans_HashMap.hmap_get_make in E; congruence.
+    + intros c Hc Hs.
+      rewrite config_HashSet.hmap_get_make in Hc. congruence.
+  - apply config_HashSet.hmap_make_WF.
+Qed.
+
+
+
+Lemma dfa_add_trans_match x y z dfa l0 l':
+  dfa_trans_HashMap.hmap_WF dfa ->
+  dfa_trans_HashMap.hmap_get (x, y) dfa = None ->
+  dfa_match dfa l0 l' ->
+  dfa_match (dfa_trans_HashMap.hmap_set (x, y) z dfa) l0 l'.
+Proof.
+  intros Hwf Hn.
+  gen l'.
+  induction l0; intros l' H.
+  - inverts H.
+    apply dfa_match_O.
+  - inversion H; subst.
+    eapply dfa_match_S.
+    + apply IHl0,H2.
+    + destruct (dfa_trans_Hash.K_eq_spec (x0,a) (x,y)).
+      * inverts e.
+        unfold Uint63_K.K in Hn.
+        congruence.
+      * rewrite dfa_trans_HashMap.hmap_get_set_other; auto.
+Qed.
+
+Lemma get_cs'_spec x y c ls a0:
+  In c ls ->
+  get_cs' x y ls = Some a0 ->
+  exists y',
+    tm (c.(s), y) = Some y' /\
+    In (x, y, y', c) a0.
+Proof.
+  gen a0.
+  unfold get_cs'.
+  induction ls; intros a0.
+  1: cbn; tauto.
+  intros [H|H].
+  - subst a.
+    cbn[fold_right].
+    unfold if_Some.
+    do 2 match goal with
+    | |- (match ?a with _ => _ end = _ -> _) => destruct a; try congruence
+    end.
+    intros H. inverts H.
+    eexists.
+    split; cbn; auto.
+  - cbn[fold_right].
+    match goal with
+    | |- ?a &&& _ = _ -> _ => destruct a eqn:E
+    end.
+    2: unfold if_Some; congruence.
+    specialize (IHls l0 H (eq_refl _)).
+    unfold if_Some.
+    destruct (tm (s a, y)); try congruence.
+    intros H0. inverts H0.
+    destruct IHls as [y' [H1 H2]].
+    exists y'.
+    split.
+    1: apply H1.
+    right. apply H2.
+Qed.
+
+
+Lemma dfa_add_trans_WF st x y sgn:
+dfa_trans_HashMap.hmap_get (x,y) (get_dfa st sgn).(trans) = None ->
+  CTL_state_WF st ->
+  match dfa_add_trans st x y sgn with
+  | None => True
+  | Some st' =>
+    CTL_state_WF st'
+  end.
+Proof.
+  intros Hn Hwf.
+  unfold dfa_add_trans,if_Some.
+  destruct (IdAllocK.get_key x (id_alloc (get_dfa st sgn))) eqn:Eia; trivial.
+  destruct (dfa_trans k y sgn (global_state st)) as [z' gs] eqn:Edt.
+  destruct (IdAllocK.get_or_alloc_id z' (id_alloc (get_dfa st sgn))) as [[z id_alloc']|] eqn:Eia2; trivial.
+  destruct (get_cs' x y (config_Index.hmap_get z (config_idx (get_dfa st sgn)))) as [a0|] eqn:Ecs'; trivial.
+  destruct Hwf.
+  constructor.
+  - destruct HO as [HO|[c1' HO]].
+    1: tauto.
+    right.
+    exists c1'.
+    destruct HO.
+    constructor.
+    + destruct H_is_config.
+      * constructor.
+        -- destruct sgn; cbn[ldfa]; cbn[trans]; cbn[get_dfa].
+          ++ apply dfa_add_trans_match; try assumption.
+            destruct HL; assumption.
+          ++ assumption.
+        -- destruct sgn; cbn[rdfa]; cbn[trans]; cbn[get_dfa].
+          ++ assumption.
+          ++ apply dfa_add_trans_match; try assumption.
+            destruct HR; assumption.
+      * constructor.
+        -- destruct sgn; cbn[ldfa]; cbn[trans]; cbn[get_dfa].
+          ++ apply dfa_add_trans_match; try assumption.
+            destruct HL; assumption.
+          ++ assumption.
+        -- destruct sgn; cbn[rdfa]; cbn[trans]; cbn[get_dfa].
+          ++ assumption.
+          ++ apply dfa_add_trans_match; try assumption.
+            destruct HR; assumption.
+    + assumption.
+  - cbn[config_set].
+    intros c1' H x0 y0.
+    specialize (HS c1' H x0 y0).
+    destruct c1' as [l0 r0 s2 sgn0].
+    cbn[trans]. cbn[config_queue].
+    destruct sgn0; cbn[get_dfa].
+    + cbn[ldfa].
+      destruct sgn.
+      * cbn[trans].
+        destruct (dfa_trans_Hash.K_eq_spec (x0,y0) (x,y)).
+        1: {
+          inverts e.
+          inverts HL.
+          rewrite dfa_trans_HashMap.hmap_get_set_same; auto 1.
+          intros E. inverts E.
+          cbn[get_dfa] in Ecs'.
+          specialize (H_config_idx _ H (eq_refl _)).
+          cbn in H_config_idx.
+          destruct (get_cs'_spec _ _ _ _ _ H_config_idx Ecs') as [y' [H2 H3]].
+          exists y'.
+          split. 1: apply H2.
+          left. rewrite in_app_iff. left. apply H3.
+        }
+        rewrite dfa_trans_HashMap.hmap_get_set_other; auto 1.
+        2: inverts HL; auto 1.
+        intros H0.
+        specialize (HS H0).
+        cbn[config_queue].
+        destruct HS as [y' [HS1 HS2]].
+        exists y'.
+        split. 1: apply HS1.
+        destruct HS2 as [HS2|[c2' [HS2 HS3]]].
+        1: left; rewrite in_app_iff; tauto.
+        right.
+        exists c2'.
+        split. 2: apply HS3.
+        gen HS2.
+        unfold next_config.
+        cbn[dir_rev]. cbn[get_dfa]. cbn[ldfa]. cbn[rdfa]. cbn[trans].
+        destruct y' as [[y1 sgn1] s1].
+        destruct sgn1; cbn[DirHash.K_eq]. 1: tauto.
+        unfold if_Some.
+        destruct (dfa_trans_HashMap.hmap_get (x0, y1) (trans (ldfa st))) eqn:E;
+        unfold Uint63_K.K,Uint63_V.V in E;
+        rewrite E.
+        2: congruence.
+        destruct (dfa_trans_Hash.K_eq_spec (x0,y1) (x,y)).
+        -- inverts e. cbn in Hn. unfold Uint63_K.K,SymHash.K in Hn. congruence.
+        -- destruct HL; rewrite dfa_trans_HashMap.hmap_get_set_other; auto 1.
+          rewrite E. tauto.
+      * intros H0.
+        specialize (HS H0).
+        cbn[config_queue].
+        destruct HS as [y' [HS1 HS2]].
+        exists y'.
+        split. 1: apply HS1.
+        destruct HS2 as [HS2|[c2' [HS2 HS3]]].
+        1: left; rewrite in_app_iff; tauto.
+        right.
+        exists c2'.
+        split. 2: apply HS3.
+        gen HS2.
+        unfold next_config.
+        cbn[dir_rev]. cbn[get_dfa]. cbn[ldfa]. cbn[rdfa]. cbn[trans].
+        destruct y' as [[y1 sgn1] s1].
+        destruct sgn1; cbn[DirHash.K_eq]. 2: tauto.
+        unfold if_Some.
+        destruct (dfa_trans_HashMap.hmap_get (l0, y1) (trans (rdfa st))) eqn:E.
+        2: congruence.
+        destruct (dfa_trans_Hash.K_eq_spec (l0,y1) (x,y)).
+        -- inverts e. cbn in Hn. unfold Uint63_K.K,SymHash.K in Hn. congruence.
+        -- destruct HR; rewrite dfa_trans_HashMap.hmap_get_set_other; auto 1.
+          rewrite E. tauto.
+    + cbn[rdfa].
+      destruct sgn.
+      * intros H0.
+        specialize (HS H0).
+        cbn[config_queue].
+        destruct HS as [y' [HS1 HS2]].
+        exists y'.
+        split. 1: apply HS1.
+        destruct HS2 as [HS2|[c2' [HS2 HS3]]].
+        1: left; rewrite in_app_iff; tauto.
+        right.
+        exists c2'.
+        split. 2: apply HS3.
+        gen HS2.
+        unfold next_config.
+        cbn[dir_rev]. cbn[get_dfa]. cbn[ldfa]. cbn[rdfa]. cbn[trans].
+        destruct y' as [[y1 sgn1] s1].
+        destruct sgn1; cbn[DirHash.K_eq]. 1: tauto.
+        unfold if_Some.
+        destruct (dfa_trans_HashMap.hmap_get (l0, y1) (trans (ldfa st))) eqn:E.
+        2: congruence.
+        destruct (dfa_trans_Hash.K_eq_spec (l0,y1) (x,y)).
+        -- inverts e. cbn in Hn. unfold Uint63_K.K,SymHash.K in Hn. congruence.
+        -- destruct HL; rewrite dfa_trans_HashMap.hmap_get_set_other; auto 1.
+          rewrite E. tauto.
+      * cbn[trans].
+        destruct (dfa_trans_Hash.K_eq_spec (x0,y0) (x,y)).
+        1: {
+          inverts e.
+          inverts HR.
+          rewrite dfa_trans_HashMap.hmap_get_set_same; auto 1.
+          intros E. inverts E.
+          cbn[get_dfa] in Ecs'.
+          specialize (H_config_idx _ H (eq_refl _)).
+          cbn in H_config_idx.
+          destruct (get_cs'_spec _ _ _ _ _ H_config_idx Ecs') as [y' [H2 H3]].
+          exists y'.
+          split. 1: apply H2.
+          left. rewrite in_app_iff. left. apply H3.
+        }
+        rewrite dfa_trans_HashMap.hmap_get_set_other; auto 1.
+        2: inverts HR; auto 1.
+        intros H0.
+        specialize (HS H0).
+        cbn[config_queue].
+        destruct HS as [y' [HS1 HS2]].
+        exists y'.
+        split. 1: apply HS1.
+        destruct HS2 as [HS2|[c2' [HS2 HS3]]].
+        1: left; rewrite in_app_iff; tauto.
+        right.
+        exists c2'.
+        split. 2: apply HS3.
+        gen HS2.
+        unfold next_config.
+        cbn[dir_rev]. cbn[get_dfa]. cbn[ldfa]. cbn[rdfa]. cbn[trans].
+        destruct y' as [[y1 sgn1] s1].
+        destruct sgn1; cbn[DirHash.K_eq]. 2: tauto.
+        unfold if_Some.
+        destruct (dfa_trans_HashMap.hmap_get (x0, y1) (trans (rdfa st))) eqn:E;
+        unfold Uint63_K.K,Uint63_V.V in E;
+        rewrite E.
+        2: congruence.
+        destruct (dfa_trans_Hash.K_eq_spec (x0,y1) (x,y)).
+        -- inverts e. cbn in Hn. unfold Uint63_K.K,SymHash.K in Hn. congruence.
+        -- destruct HR; rewrite dfa_trans_HashMap.hmap_get_set_other; auto 1.
+          rewrite E. tauto.
+  - cbn[ldfa].
+    inverts HL.
+    destruct sgn.
+    2: constructor; assumption.
+    constructor.
+    * cbn[id_alloc].
+      epose proof (IdAllocK.get_or_alloc_id_WF _ _ H_id_alloc_wf) as H.
+      cbn[get_dfa] in Eia2.
+      rewrite Eia2 in H.
+      apply H.
+    * cbn[trans].
+      apply dfa_trans_HashMap.hmap_set_WF; assumption.
+    * cbn[inv1_trans].
+      apply dfa_trans_inv1_HashMap.hmap_add_WF; assumption.
+    * cbn[inv2_trans].
+      apply dfa_trans_inv2_HashMap.hmap_add_WF; assumption.
+    * assumption.
+    * cbn[trans].
+      destruct (dfa_trans_Hash.K_eq_spec (int0,s0) (x,y)).
+      -- rewrite <-e in Hn. cbn[get_dfa] in Hn.
+        congruence.
+      -- rewrite dfa_trans_HashMap.hmap_get_set_other; assumption.
+    * cbn[trans]. cbn[inv1_trans].
+      intros x0 y0 z0.
+      destruct (dfa_trans_Hash.K_eq_spec (x0,y0) (x,y)).
+      -- inverts e.
+        rewrite dfa_trans_HashMap.hmap_get_set_same; try assumption.
+        intros Hz; inverts Hz.
+        rewrite dfa_trans_inv1_HashMap.hmap_get_add_same; try assumption.
+        left. reflexivity.
+      -- rewrite dfa_trans_HashMap.hmap_get_set_other; try assumption.
+        intros H.
+        specialize (H_inv1_trans x0 y0 z0 H).
+        apply dfa_trans_inv1_HashMap.hmap_get_add_mono; assumption.
+    * cbn[trans]. cbn[inv2_trans].
+      intros x0 y0 z0.
+      destruct (dfa_trans_Hash.K_eq_spec (x0,y0) (x,y)).
+      -- inverts e.
+        rewrite dfa_trans_HashMap.hmap_get_set_same; try assumption.
+        intros Hz; inverts Hz.
+        rewrite dfa_trans_inv2_HashMap.hmap_get_add_same; try assumption.
+        left. reflexivity.
+      -- rewrite dfa_trans_HashMap.hmap_get_set_other; try assumption.
+        intros H.
+        specialize (H_inv2_trans x0 y0 z0 H).
+        apply dfa_trans_inv2_HashMap.hmap_get_add_mono; assumption.
+    * assumption.
+  - cbn[rdfa].
+    inverts HR.
+    destruct sgn.
+    1: constructor; assumption.
+    constructor.
+    * cbn[id_alloc].
+      epose proof (IdAllocK.get_or_alloc_id_WF _ _ H_id_alloc_wf) as H.
+      cbn[get_dfa] in Eia2.
+      rewrite Eia2 in H.
+      apply H.
+    * cbn[trans].
+      apply dfa_trans_HashMap.hmap_set_WF; assumption.
+    * cbn[inv1_trans].
+      apply dfa_trans_inv1_HashMap.hmap_add_WF; assumption.
+    * cbn[inv2_trans].
+      apply dfa_trans_inv2_HashMap.hmap_add_WF; assumption.
+    * assumption.
+    * cbn[trans].
+      destruct (dfa_trans_Hash.K_eq_spec (int0,s0) (x,y)).
+      -- rewrite <-e in Hn. cbn[get_dfa] in Hn.
+        congruence.
+      -- rewrite dfa_trans_HashMap.hmap_get_set_other; assumption.
+    * cbn[trans]. cbn[inv1_trans].
+      intros x0 y0 z0.
+      destruct (dfa_trans_Hash.K_eq_spec (x0,y0) (x,y)).
+      -- inverts e.
+        rewrite dfa_trans_HashMap.hmap_get_set_same; try assumption.
+        intros Hz; inverts Hz.
+        rewrite dfa_trans_inv1_HashMap.hmap_get_add_same; try assumption.
+        left. reflexivity.
+      -- rewrite dfa_trans_HashMap.hmap_get_set_other; try assumption.
+        intros H.
+        specialize (H_inv1_trans x0 y0 z0 H).
+        apply dfa_trans_inv1_HashMap.hmap_get_add_mono; assumption.
+    * cbn[trans]. cbn[inv2_trans].
+      intros x0 y0 z0.
+      destruct (dfa_trans_Hash.K_eq_spec (x0,y0) (x,y)).
+      -- inverts e.
+        rewrite dfa_trans_HashMap.hmap_get_set_same; try assumption.
+        intros Hz; inverts Hz.
+        rewrite dfa_trans_inv2_HashMap.hmap_get_add_same; try assumption.
+        left. reflexivity.
+      -- rewrite dfa_trans_HashMap.hmap_get_set_other; try assumption.
+        intros H.
+        specialize (H_inv2_trans x0 y0 z0 H).
+        apply dfa_trans_inv2_HashMap.hmap_get_add_mono; assumption.
+    * assumption.
+  - assumption.
+Qed.
+
+Lemma CTL_add_side_WF st sgn0 ls:
+  CTL_state_WF st ->
+  match CTL_add_side st sgn0 ls with
+  | None => True
+  | Some (st',_) => CTL_state_WF st'
+  end.
+Proof.
+  intros H.
+  unfold CTL_add_side.
+  induction ls.
+  1: apply H.
+  cbn[fold_right].
+  match goal with
+  | |- match ?a &&& _ with _ => _ end => destruct a as [[st' z]|]; trivial
+  end.
+  unfold if_Some.
+  destruct (dfa_get_trans st' z a sgn0) eqn:E; auto 1.
+  pose proof (dfa_add_trans_WF st' z a sgn0 E IHls).
+  destruct (dfa_add_trans st' z a sgn0); trivial.
+  destruct (dfa_get_trans c z a sgn0); trivial.
+Qed.
+
+Lemma CTL_state_1_WF cfg len:
+  match CTL_state_1 cfg len with
+  | None => True
+  | Some st => CTL_state_WF st
+  end.
+Proof.
+  unfold CTL_state_1.
+  destruct (DH_config_init) as [[[l0 r0] s2] sgn0].
+  unfold if_Some.
+  pose proof (CTL_state_0_WF cfg len).
+  destruct (CTL_state_0 cfg len); trivial.
+  pose proof (CTL_add_side_WF c (dir_rev sgn0) l0 H).
+  destruct (CTL_add_side c (dir_rev sgn0) l0) as [[st _]|]; trivial.
+  pose proof (CTL_add_side_WF st sgn0 r0 H0).
+  destruct (CTL_add_side st sgn0 r0) as [[st0 _]|]; trivial.
+Qed.
+
+Lemma CTL_match_side_WF st sgn0 ls:
+  CTL_state_WF st ->
+  match CTL_match_side st sgn0 ls with
+  | None => True
+  | Some z => dfa_match (get_dfa st sgn0).(trans) ls z
+  end.
+Proof.
+  intros H.
+  unfold CTL_match_side.
+  induction ls.
+  1: constructor.
+  cbn[fold_right].
+  match goal with
+  | |- match ?a &&& _ with _ => _ end => destruct a as [z|]; trivial
+  end.
+  unfold if_Some.
+  destruct (dfa_get_trans st z a sgn0) eqn:E; auto 1.
+  eapply dfa_match_S; eauto.
+Qed.
+
+
+
+Lemma dfa_add_config_trans dfa sgn0 c:
+  ((dfa_add_config dfa sgn0 c).(trans)) = (dfa.(trans)).
+Proof.
+  unfold dfa_add_config.
+  destruct (DirHash.K_eq (sgn c) sgn0); reflexivity.
+Qed.
+Lemma dfa_add_config_inv1_trans dfa sgn0 c:
+  ((dfa_add_config dfa sgn0 c).(inv1_trans)) = (dfa.(inv1_trans)).
+Proof.
+  unfold dfa_add_config.
+  destruct (DirHash.K_eq (sgn c) sgn0); reflexivity.
+Qed.
+Lemma dfa_add_config_inv2_trans dfa sgn0 c:
+  ((dfa_add_config dfa sgn0 c).(inv2_trans)) = (dfa.(inv2_trans)).
+Proof.
+  unfold dfa_add_config.
+  destruct (DirHash.K_eq (sgn c) sgn0); reflexivity.
+Qed.
+
+Lemma dfa_add_config_id_alloc dfa sgn0 c:
+  ((dfa_add_config dfa sgn0 c).(id_alloc)) = (dfa.(id_alloc)).
+Proof.
+  unfold dfa_add_config.
+  destruct (DirHash.K_eq (sgn c) sgn0); reflexivity.
+Qed.
+
+Lemma get_cs''_spec x y c ls l0:
+In (x, y) ls ->
+get_cs'' c ls = Some l0 ->
+exists y' : Sym * dir * Q,
+  tm (c.(s), y) = Some y' /\
+  In (x, y, y', c) l0.
+Proof.
+  unfold get_cs''.
+  gen l0.
+  induction ls; intros l0.
+  - cbn. tauto.
+  - intros [H|H].
+    + subst a.
+      unfold if_Some.
+      cbn.
+      do 2 match goal with
+      | |- (match ?a with _ => _ end = _ -> _) => destruct a; try congruence
+      end.
+      intros H. inverts H.
+      eexists.
+      split; cbn; auto.
+    + destruct a as [x0 y0].
+      cbn[fold_right].
+      match goal with
+      | |- ?a &&& _ = _ -> _ => destruct a eqn:E
+      end.
+      2: unfold if_Some; congruence.
+      specialize (IHls l1 H (eq_refl _)).
+      unfold if_Some.
+      destruct (tm (s c, y0)); try congruence.
+      intros H0. inverts H0.
+      destruct IHls as [y' [H1 H2]].
+      exists y'.
+      split.
+      1: apply H1.
+      right. apply H2.
+Qed.
+
+Lemma CTL_state_init_WF cfg len:
+  match CTL_state_init cfg len with
+  | Some st' => CTL_state_WF st'
+  | None => True
+  end.
+Proof.
+  unfold CTL_state_init.
+  destruct DH_config_init as [[[l0 r0] s2] sgn0] eqn:Edci.
+  unfold if_Some.
+  pose proof (CTL_state_1_WF cfg len) as H1.
+  destruct (CTL_state_1 cfg len) as [st|]; trivial.
+  pose proof (CTL_match_side_WF st (dir_rev sgn0) l0 H1) as H2.
+  destruct (CTL_match_side st (dir_rev sgn0) l0) as [l1|]; trivial.
+  pose proof (CTL_match_side_WF st sgn0 r0 H1) as H3.
+  destruct (CTL_match_side st sgn0 r0) as [r1|]; trivial.
+  cbn[r]. cbn[sgn].
+  cbn[get_dfa].
+  remember ((dfa_trans_inv2_HashMap.hmap_get r1 (inv2_trans (get_dfa st sgn0)))) as ls.
+  destruct (get_cs'' {| l := l1; r := r1; s := s2; sgn := sgn0 |} ls) eqn:E1; trivial.
+  destruct H1.
+  constructor.
+  - right.
+    exists {| l := l1; r := r1; s := s2; sgn := sgn0 |}.
+    unfold config_init.
+    rewrite Edci.
+    constructor.
+    + destruct sgn0;
+      constructor; assumption.
+    + apply config_HashSet.hmap_get_set_same; assumption.
+  - cbn_proj.
+    intros c1' Hc1'.
+    destruct (config_Hash.K_eq_spec c1' {| l := l1; r := r1; s := s2; sgn := sgn0 |}),sgn0.
+    + subst c1'. cbn[get_dfa]. cbn_proj.
+      rewrite dfa_add_config_trans.
+      intros x y H.
+      epose proof (get_cs''_spec _ _ _ _ _ _ E1) as H0.
+      destruct H0 as [y' [H0 H1]].
+      exists y'.
+      split. 1: apply H0.
+      left. rewrite in_app_iff. left. apply H1.
+      Unshelve.
+      subst ls.
+      gen H.
+      inverts HL.
+      apply H_inv2_trans.
+    + subst c1'. cbn[get_dfa]. cbn_proj.
+      rewrite dfa_add_config_trans.
+      intros x y H.
+      epose proof (get_cs''_spec _ _ _ _ _ _ E1) as H0.
+      destruct H0 as [y' [H0 H1]].
+      exists y'.
+      split. 1: apply H0.
+      left. rewrite in_app_iff. left. apply H1.
+      Unshelve.
+      subst ls.
+      gen H.
+      inverts HR.
+      apply H_inv2_trans.
+    + rewrite config_HashSet.hmap_get_set_other in Hc1'; auto 1.
+      intros x y.
+      specialize (HS c1' Hc1' x y).
+      destruct c1' as [l3 r2 s3 sgn0].
+      intros H.
+      unshelve epose proof (HS _) as HS.
+      {
+        gen H.
+        destruct sgn0; cbn[get_dfa]; cbn_proj;
+        rewrite dfa_add_config_trans; tauto.
+      }
+      destruct HS as [y' [HS1 HS2]].
+      exists y'.
+      split. 1: apply HS1.
+      destruct HS2 as [HS2|HS2].
+      * left. rewrite in_app_iff. tauto.
+      * right. destruct HS2 as [c2' [HS2 HS3]].
+        exists c2'. split.
+        -- gen HS2.
+          unfold next_config.
+          destruct y' as [[y1 sgn1] s1].
+          destruct (DirHash.K_eq_spec sgn0 sgn1);
+          destruct sgn0;
+          cbn[dir_rev]; cbn[get_dfa]; cbn[ldfa]; cbn[rdfa];
+          rewrite dfa_add_config_trans;
+          tauto.
+        -- gen HS3.
+          destruct (config_Hash.K_eq_spec c2' {| l := l1; r := r1; s := s2; sgn := L |}).
+          ++ subst c2'.
+            rewrite config_HashSet.hmap_get_set_same; auto 1.
+          ++ rewrite config_HashSet.hmap_get_set_other; auto 1.
+    + rewrite config_HashSet.hmap_get_set_other in Hc1'; auto 1.
+      intros x y.
+      specialize (HS c1' Hc1' x y).
+      destruct c1' as [l3 r2 s3 sgn0].
+      intros H.
+      unshelve epose proof (HS _) as HS.
+      {
+        gen H.
+        destruct sgn0; cbn[get_dfa]; cbn_proj;
+        rewrite dfa_add_config_trans; tauto.
+      }
+      destruct HS as [y' [HS1 HS2]].
+      exists y'.
+      split. 1: apply HS1.
+      destruct HS2 as [HS2|HS2].
+      * left. rewrite in_app_iff. tauto.
+      * right. destruct HS2 as [c2' [HS2 HS3]].
+        exists c2'. split.
+        -- gen HS2.
+          unfold next_config.
+          destruct y' as [[y1 sgn1] s1].
+          destruct (DirHash.K_eq_spec sgn0 sgn1);
+          destruct sgn0;
+          cbn[dir_rev]; cbn[get_dfa]; cbn[ldfa]; cbn[rdfa];
+          rewrite dfa_add_config_trans;
+          tauto.
+        -- gen HS3.
+          destruct (config_Hash.K_eq_spec c2' {| l := l1; r := r1; s := s2; sgn := R |}).
+          ++ subst c2'.
+            rewrite config_HashSet.hmap_get_set_same; auto 1.
+          ++ rewrite config_HashSet.hmap_get_set_other; auto 1.
+  - destruct sgn0.
+    -- cbn_proj.
+      inverts HL.
+      constructor; try assumption;
+      cbn_proj.
+      + unfold dfa_add_config.
+        cbn[sgn]. cbn[DirHash.K_eq].
+        cbn_proj.
+        apply config_Index.hmap_add_WF; assumption.
+      + unfold dfa_add_config.
+        cbn[sgn]. cbn[DirHash.K_eq].
+        cbn_proj.
+        intros c Hc Hs.
+        destruct (config_Hash.K_eq_spec c {| l := l1; r := r1; s := s2; sgn := L |}).
+        * subst c.
+          rewrite config_Index.hmap_get_add_same; cbn; auto 2.
+        * rewrite config_HashSet.hmap_get_set_other in Hc; try assumption.
+          apply config_Index.hmap_get_add_mono; auto 1.
+          apply H_config_idx; auto 1.
+    -- cbn_proj.
+      inverts HL.
+      constructor; try assumption.
+      cbn_proj.
+      intros c Hc Hs.
+      rewrite config_HashSet.hmap_get_set_other in Hc; try assumption.
+      2: destruct c; cbn in Hs; congruence.
+      apply H_config_idx; auto 1.
+  - destruct sgn0.
+    -- cbn_proj.
+      inverts HR.
+      constructor; try assumption.
+      cbn_proj.
+      intros c Hc Hs.
+      rewrite config_HashSet.hmap_get_set_other in Hc; try assumption.
+      2: destruct c; cbn in Hs; congruence.
+      apply H_config_idx; auto 1.
+    -- cbn_proj.
+      inverts HR.
+      constructor; try assumption;
+      cbn_proj.
+      + unfold dfa_add_config.
+        cbn[sgn]. cbn[DirHash.K_eq].
+        cbn_proj.
+        apply config_Index.hmap_add_WF; assumption.
+      + unfold dfa_add_config.
+        cbn[sgn]. cbn[DirHash.K_eq].
+        cbn_proj.
+        intros c Hc Hs.
+        destruct (config_Hash.K_eq_spec c {| l := l1; r := r1; s := s2; sgn := R |}).
+        * subst c.
+          rewrite config_Index.hmap_get_add_same; cbn; auto 2.
+        * rewrite config_HashSet.hmap_get_set_other in Hc; try assumption.
+          apply config_Index.hmap_get_add_mono; auto 1.
+          apply H_config_idx; auto 1.
+  - cbn_proj.
+    apply config_HashSet.hmap_set_WF; assumption.
+Qed.
+
+Lemma config_push_WF st c1':
+  CTL_state_WF st ->
+  (forall h t, st.(config_queue) = h::t ->
+  next_config h st = Some c1' ->
+  match config_push st c1' with
+  | Some st' => CTL_state_WF st'
+  | None => True
+  end).
+Proof.
+  intros Hwf h t Hq Hnx.
+  unfold config_push.
+  rewrite config_HashSet.hmap_add_spec.
+  destruct (config_HashSet.hmap_get c1' (config_set st)) eqn:E.
+  - destruct Hwf.
+    constructor.
+    + destruct HO as [HO|[c' HO]].
+      1: tauto.
+      right.
+      exists c'.
+      destruct HO.
+      constructor.
+      * destruct H_is_config;
+        constructor; assumption.
+      * assumption.
+    + intros c' H x y.
+      specialize (HS c' H x y).
+      destruct c' as [l0 r0 s0 sgn0].
+      intros H0.
+      specialize (HS H0).
+      destruct HS as [y' [HS1 HS2]].
+      exists y'.
+      split. 1: apply HS1.
+      destruct HS2 as [HS2|HS2].
+      2: right; apply HS2.
+      rewrite Hq in HS2.
+      rewrite Hq.
+      cbn in HS2.
+      destruct HS2 as [HS2|HS2].
+      2: left; apply HS2.
+      right.
+      exists c1'.
+      subst h.
+      split. 1: apply Hnx.
+      destruct v.
+      apply E.
+    + cbn.
+      destruct HL.
+      constructor; try assumption.
+    + cbn.
+      destruct HR.
+      constructor; try assumption.
+    + assumption.
+  - destruct Hwf.
+    unfold if_Some.
+    destruct (get_cs'' c1' (dfa_trans_inv2_HashMap.hmap_get (r c1') (inv2_trans (get_dfa st (sgn c1'))))) eqn:Ecs''; trivial.
+    constructor.
+    + destruct HO as [HO|[c' HO]].
+      1: tauto.
+      right.
+      exists c'.
+      destruct HO.
+      constructor.
+      * destruct H_is_config; constructor;
+        cbn; rewrite dfa_add_config_trans; assumption.
+      * cbn[config_set].
+        destruct (config_Hash.K_eq_spec c1'0 c1').
+        -- subst. apply config_HashSet.hmap_get_set_same; assumption.
+        -- rewrite config_HashSet.hmap_get_set_other; assumption.
+    + intros c' H x y.
+      cbn[config_set] in H.
+      destruct (config_Hash.K_eq_spec c' c1').
+      1:{
+        subst c'.
+        destruct c1' as [l1 r0 s2 sgn0].
+        cbn[config_queue].
+        cbn in Ecs''.
+        intros H0.
+        assert (dfa_trans_HashMap.hmap_get (x, y) (get_dfa st sgn0).(trans) = Some r0) as H0'. {
+          applys_eq H0.
+          destruct sgn0; cbn[get_dfa]; cbn[ldfa]; cbn[rdfa];
+          rewrite dfa_add_config_trans;
+          reflexivity.
+        }
+        clear H0.
+        remember (dfa_trans_inv2_HashMap.hmap_get r0 (inv2_trans (get_dfa st sgn0))) as ls.
+        assert (In (x,y) ls) as H1'. {
+          subst ls.
+          gen H0'.
+          destruct sgn0; cbn[get_dfa].
+          - destruct HL.
+            apply H_inv2_trans.
+          - destruct HR.
+            apply H_inv2_trans.
+        }
+        destruct (get_cs''_spec _ _ _ _ _ H1' Ecs'') as [y' [H2 H3]].
+        exists y'.
+        split. 1: apply H2.
+        left.
+        rewrite in_app_iff. tauto.
+      }
+      unshelve epose proof (HS c' _ x y) as HS.
+      1: rewrite config_HashSet.hmap_get_set_other in H; assumption.
+      destruct c' as [l1 r0 s2 sgn0] eqn:Ec'.
+      intros H0.
+      unshelve epose proof (HS _) as HS.
+      1: destruct sgn0; cbn in H0; rewrite dfa_add_config_trans in H0; apply H0.
+      destruct HS as [y' [HS1 HS2]].
+      exists y'.
+      split. 1: apply HS1.
+      destruct HS2 as [HS2|HS2].
+      2: {
+        destruct HS2 as [c2' [HS2 HS3]].
+        cbn[config_set].
+        right.
+        exists c2'.
+        split. 2: {
+          destruct (config_Hash.K_eq_spec c2' c1').
+          - subst c2'.
+            apply config_HashSet.hmap_get_set_same; assumption.
+          - rewrite config_HashSet.hmap_get_set_other; assumption.
+        }
+        gen HS2.
+        unfold next_config.
+        destruct y' as [[y1 sgn1] s1].
+        destruct (DirHash.K_eq_spec sgn0 sgn1);
+        destruct sgn0;
+        cbn[dir_rev]; cbn[get_dfa]; cbn[ldfa]; cbn[rdfa];
+        rewrite dfa_add_config_trans;
+        tauto.
+      }
+      rewrite Hq in HS2.
+      rewrite Hq.
+      cbn in HS2.
+      cbn[config_queue].
+      cbn[config_set].
+      cbn[tl].
+      destruct HS2 as [HS2|HS2].
+      2: left; rewrite in_app_iff; right; apply HS2.
+      right.
+      exists c1'.
+      subst h.
+      split.
+      2: apply config_HashSet.hmap_get_set_same; assumption.
+      gen Hnx.
+      unfold next_config.
+      destruct y' as [[y1 sgn1] s1].
+      destruct (DirHash.K_eq_spec sgn0 sgn1);
+      destruct sgn0;
+      cbn[dir_rev]; cbn[get_dfa]; cbn[ldfa]; cbn[rdfa];
+      rewrite dfa_add_config_trans;
+      tauto.
+    + cbn[ldfa].
+      inverts HL.
+      constructor.
+      all: repeat (
+      rewrite dfa_add_config_id_alloc ||
+      rewrite dfa_add_config_trans ||
+      rewrite dfa_add_config_inv1_trans ||
+      rewrite dfa_add_config_inv2_trans); try assumption.
+      * unfold dfa_add_config.
+        destruct (DirHash.K_eq (sgn c1') L).
+        2: assumption.
+        apply config_Index.hmap_add_WF; assumption.
+      * cbn[config_set].
+        intros c Hc Hs.
+        unfold dfa_add_config.
+        destruct (DirHash.K_eq_spec (sgn c1') L).
+        -- cbn[config_idx].
+          destruct (config_Hash.K_eq_spec c c1').
+          ++ subst c.
+            rewrite config_Index.hmap_get_add_same; auto 1.
+            left; reflexivity.
+          ++ destruct (Uint63_K.K_eq_spec (r c) (r c1')).
+            ** rewrite <-e0.
+              rewrite config_Index.hmap_get_add_same; auto 1.
+              right.
+              apply H_config_idx; auto 1.
+              rewrite config_HashSet.hmap_get_set_other in Hc; assumption.
+            ** rewrite config_Index.hmap_get_add_other; auto 1.
+              apply H_config_idx; auto 1.
+              rewrite config_HashSet.hmap_get_set_other in Hc; assumption.
+        -- apply H_config_idx; auto.
+          destruct (config_Hash.K_eq_spec c c1').
+          1: congruence.
+          rewrite config_HashSet.hmap_get_set_other in Hc; assumption.
+    + cbn[rdfa].
+      inverts HR.
+      constructor.
+      all: repeat (
+      rewrite dfa_add_config_id_alloc ||
+      rewrite dfa_add_config_trans ||
+      rewrite dfa_add_config_inv1_trans ||
+      rewrite dfa_add_config_inv2_trans); try assumption.
+      * unfold dfa_add_config.
+        destruct (DirHash.K_eq (sgn c1') R).
+        2: assumption.
+        apply config_Index.hmap_add_WF; assumption.
+      * cbn[config_set].
+        intros c Hc Hs.
+        unfold dfa_add_config.
+        destruct (DirHash.K_eq_spec (sgn c1') R).
+        -- cbn[config_idx].
+          destruct (config_Hash.K_eq_spec c c1').
+          ++ subst c.
+            rewrite config_Index.hmap_get_add_same; auto 1.
+            left; reflexivity.
+          ++ destruct (Uint63_K.K_eq_spec (r c) (r c1')).
+            ** rewrite <-e0.
+              rewrite config_Index.hmap_get_add_same; auto 1.
+              right.
+              apply H_config_idx; auto 1.
+              rewrite config_HashSet.hmap_get_set_other in Hc; assumption.
+            ** rewrite config_Index.hmap_get_add_other; auto 1.
+              apply H_config_idx; auto 1.
+              rewrite config_HashSet.hmap_get_set_other in Hc; assumption.
+        -- apply H_config_idx; auto.
+          destruct (config_Hash.K_eq_spec c c1').
+          1: congruence.
+          rewrite config_HashSet.hmap_get_set_other in Hc; assumption.
+    + cbn[config_set].
+      apply config_HashSet.hmap_set_WF; assumption.
+Qed.
+
+Lemma CTL_step_WF st:
+CTL_state_WF st ->
+match CTL_step st with
+| None => True
+| Some st' =>
+  CTL_state_WF st'
+end.
+Proof.
+unfold CTL_step.
+destruct (config_queue st) as [|q1 q0] eqn:Eq; trivial.
+destruct q1 as [[[x y] y'] c1'].
+destruct c1' as [l0 r0 s0 sgn0].
+destruct y' as [[y1 sgn1] s2].
+destruct sgn0,sgn1; cbn.
+- destruct (dfa_trans_HashMap.hmap_get (l0, y1) (trans (rdfa st))) eqn:E.
+  + intros Hwf.
+    eapply config_push_WF; eauto.
+    cbn. unfold if_Some. rewrite E. reflexivity.
+  + apply (dfa_add_trans_WF st _ _ R E).
+- destruct (dfa_trans_HashMap.hmap_get (x, y1) (trans (ldfa st))) eqn:E.
+  + intros Hwf.
+    eapply config_push_WF; eauto.
+    cbn. unfold if_Some. rewrite E. reflexivity.
+  + apply (dfa_add_trans_WF st _ _ L E).
+- destruct (dfa_trans_HashMap.hmap_get (x, y1) (trans (rdfa st))) eqn:E.
+  + intros Hwf.
+    eapply config_push_WF; eauto.
+    cbn. unfold if_Some. rewrite E. reflexivity.
+  + apply (dfa_add_trans_WF st _ _ R E).
+- destruct (dfa_trans_HashMap.hmap_get (l0, y1) (trans (ldfa st))) eqn:E.
+  + intros Hwf.
+    eapply config_push_WF; eauto.
+    cbn. unfold if_Some. rewrite E. reflexivity.
+  + apply (dfa_add_trans_WF st _ _ L E).
+Qed.
+
+Lemma CTL_state_end st:
+CTL_state_WF st ->
+st.(config_queue) = nil ->
+st.(init_flag) = true ->
+~halts tm config_init.
+Proof.
+intros Hwf Hqnil Hinit.
+destruct Hwf.
+apply step_nonhalt with (P:=fun c1 => exists c1' : config, is_config_in_mset st c1 c1').
+2: destruct HO as [HO|HO]; [congruence|apply HO].
+intros c1 [c1' HP].
+destruct HP.
+specialize (HS c1' H_in_mset).
+rewrite Hqnil in HS.
+cbn[In] in HS.
+destruct H_is_config.
+- cbn in HS.
+  destruct Hlm.
+  + remember (ldfa st) as ldfa'.
+    inverts HL.
+    specialize (HS int0 s0 H_dfa_state0).
+    destruct HS as [[[y1 sgn1] s2] [HS1 [HS2|[c2' [HS2 HS3]]]]]. 1: tauto.
+    destruct sgn1.
+    * unfold if_Some in HS2.
+      destruct (dfa_trans_HashMap.hmap_get (r', y1) (trans (rdfa st))) eqn:HS2'.
+      2: congruence.
+      inverts HS2; eexists; split.
+      -- eexists; constructor; [constructor | apply HS3].
+        1: apply dfa_match_O.
+        eapply dfa_match_S. 2: apply HS2'.  apply Hrm.
+      -- cbn.
+        applys_eq step_through.
+        1: rewrite <-const_unfold; reflexivity.
+        assumption.
+    * unfold if_Some in HS2.
+      destruct (dfa_trans_HashMap.hmap_get (int0, y1) (trans ldfa')) eqn:HS2'.
+      2: congruence.
+      inverts HS2; eexists; split.
+      -- eexists; constructor; [constructor | apply HS3].
+        2: apply Hrm.
+        rewrite <-Heqldfa'.
+        eapply dfa_match_S.
+        2: apply HS2'.
+        apply dfa_match_O.
+      -- cbn.
+        applys_eq step_back.
+        1: rewrite <-const_unfold; reflexivity.
+        1: reflexivity.
+        assumption.
+  + remember (ldfa st) as ldfa'.
+    inverts HL.
+    specialize (HS x a H).
+    destruct HS as [[[y1 sgn1] s2] [HS1 [HS2|[c2' [HS2 HS3]]]]]. 1: tauto.
+    destruct sgn1.
+    * unfold if_Some in HS2.
+      destruct (dfa_trans_HashMap.hmap_get (r', y1) (trans (rdfa st))) eqn:HS2'.
+      2: congruence.
+      inverts HS2; eexists; split.
+      -- eexists; constructor; [constructor | apply HS3].
+        1: rewrite <-Heqldfa'; apply Hlm.
+        eapply dfa_match_S; eassumption.
+      -- constructor. apply HS1.
+    * unfold if_Some in HS2.
+      destruct (dfa_trans_HashMap.hmap_get (x, y1) (trans ldfa')) eqn:HS2'.
+      2: congruence.
+      inverts HS2; eexists; split.
+      -- eexists; constructor; [constructor | apply HS3].
+        2: apply Hrm.
+        rewrite <-Heqldfa'.
+        eapply dfa_match_S; eassumption.
+      -- constructor. apply HS1.
+- cbn in HS.
+  destruct Hrm.
+  + remember (rdfa st) as rdfa'.
+    inverts HR.
+    specialize (HS int0 s0 H_dfa_state0).
+    destruct HS as [[[y1 sgn1] s2] [HS1 [HS2|[c2' [HS2 HS3]]]]]. 1: tauto.
+    destruct sgn1.
+    * unfold if_Some in HS2.
+      destruct (dfa_trans_HashMap.hmap_get (int0, y1) (trans rdfa')) eqn:HS2'.
+      2: congruence.
+      inverts HS2; eexists; split.
+      -- eexists; constructor; [constructor | apply HS3].
+        1: apply Hlm.
+        rewrite <-Heqrdfa'.
+        eapply dfa_match_S.
+        2: apply HS2'.
+        apply dfa_match_O.
+      -- cbn.
+        applys_eq step_back.
+        1: rewrite <-const_unfold; reflexivity.
+        1: reflexivity.
+        assumption.
+    * unfold if_Some in HS2.
+      destruct (dfa_trans_HashMap.hmap_get (l', y1) (trans (ldfa st))) eqn:HS2'.
+      2: congruence.
+      inverts HS2; eexists; split.
+      -- eexists; constructor; [constructor | apply HS3].
+        2: apply dfa_match_O.
+        eapply dfa_match_S; eassumption.
+      -- cbn.
+        applys_eq step_through.
+        1: rewrite <-const_unfold; reflexivity.
+        assumption.
+  + remember (rdfa st) as rdfa'.
+    inverts HR.
+    specialize (HS x a H).
+    destruct HS as [[[y1 sgn1] s2] [HS1 [HS2|[c2' [HS2 HS3]]]]]. 1: tauto.
+    destruct sgn1.
+    * unfold if_Some in HS2.
+      destruct (dfa_trans_HashMap.hmap_get (x, y1) (trans rdfa')) eqn:HS2'.
+      2: congruence.
+      inverts HS2; eexists; split.
+      -- eexists; constructor; [constructor | apply HS3].
+        1: apply Hlm.
+        rewrite <-Heqrdfa'.
+        eapply dfa_match_S; eassumption.
+      -- constructor. apply HS1.
+    * unfold if_Some in HS2.
+      destruct (dfa_trans_HashMap.hmap_get (l', y1) (trans (ldfa st))) eqn:HS2'.
+      2: congruence.
+      inverts HS2; eexists; split.
+      -- eexists; constructor; [constructor | apply HS3].
+        2: rewrite <-Heqrdfa'; apply Hrm.
+        eapply dfa_match_S; eassumption.
+      -- constructor. apply HS1.
+Qed.
+
+Lemma CTL_steps_spec cfg len T:
+match CTL_steps cfg len T with
+| inl st => CTL_state_WF st
+| inr st =>
+  match st with
+  | Some st => CTL_state_WF st
+  | None => True
+  end
+end.
+Proof.
+  unfold CTL_steps.
+  apply N_iter_until_spec.
+  - intros st Hwf.
+    pose proof (CTL_step_WF st Hwf) as H.
+    destruct (CTL_step st) as [st'|]; trivial.
+  - pose proof (CTL_state_init_WF cfg len) as H.
+    destruct (CTL_state_init cfg len); trivial.
+Qed.
+
+Lemma CTL_decide_nonhalt_spec cfg len T:
+CTL_decide_nonhalt cfg len T = true ->
+~halts tm config_init.
+Proof.
+  unfold CTL_decide_nonhalt.
+  pose proof (CTL_steps_spec cfg len T).
+  destruct (CTL_steps cfg len T) as [st|[st|]]; try congruence.
+  rewrite and_true_iff.
+  intros [H1 H2].
+  destruct (config_queue st) eqn:E; try congruence.
+  eapply CTL_state_end; eauto.
+Qed.
+
+End tm_ctx.
+
+End CTL.
+
+
+
+
+
+
+Module TMCtx(Ctx:TM.Ctx) <: Ctx.
+Include Ctx.
+End TMCtx.
+
+Module DHTMFromTM(Ctx:TM.Ctx).
+Module TMCtx := TMCtx Ctx.
+Module DHTM := DHTM TMCtx.
+Module TM := TM Ctx.
+
+Definition map_config(x:DHTM.DH_config):Ctx.Q*TM.tape :=
+match x with
+| (l,r,s,L) => (s,(Streams.tl r,Streams.hd r,l))
+| (l,r,s,R) => (s,(l,Streams.hd r,Streams.tl r))
+end.
+
+Ltac cbn_all :=
+  repeat match goal with
+  | H:_ |- _ => cbn in H || fail
+  end;
+  cbn.
+
+Lemma map_step {tm c1 c2}:
+  DHTM.step tm c1 c2 ->
+  TM.step tm (map_config c1) (map_config c2).
+Proof.
+  destruct c1 as [[[l1 r1] s1] sgn1].
+  destruct c2 as [[[l2 r2] s2] sgn2].
+  intros; unfold map_config.
+  destruct sgn1,sgn2;
+  inverts H.
+  1: destruct l1.
+  all: constructor; auto 1.
+Qed.
+
+Lemma map_multistep {tm n c1 c2}:
+  DHTM.multistep tm n c1 c2 ->
+  TM.multistep tm n (map_config c1) (map_config c2).
+Proof.
+  gen c1 c2.
+  induction n; intros c1 c2 H.
+  - inverts H.
+    constructor.
+  - inverts H.
+    pose proof (map_step H1).
+    econstructor; eauto.
+Qed.
+
+Lemma map_halts {tm}:
+  DHTM.halts' tm DHTM.c0 ->
+  TM.halts' tm TM.c0.
+Proof.
+  rewrite <-DHTM.halts_halts'.
+  rewrite <-TM.halts_halts'.
+  intros [n [c [H H0]]].
+  exists n.
+  eexists.
+  split.
+  1: apply (map_multistep H).
+  destruct c as [[[l r] s] sgn].
+  gen H0. cbn.
+  destruct r,sgn; cbn; tauto.
+Qed.
+
+Lemma map_nonhalt {tm}:
+  ~DHTM.halts' tm DHTM.c0 ->
+  ~TM.halts' tm TM.c0.
+Proof.
+  rewrite <-DHTM.halts_halts'.
+  rewrite <-TM.halts_halts'.
+  rewrite DHTM.nonhalt_iff.
+  rewrite TM.nonhalt_iff.
+  intros H n.
+  specialize (H n).
+  destruct H as [c' H].
+  eexists.
+  apply (map_multistep H).
+Qed.
+
+End DHTMFromTM.
+
+
+
+
+Module BlockTMCtx(Ctx:Ctx)<: Ctx.
+Definition Q:Type := Ctx.Q*dir.
+Definition Sym:Type := list Ctx.Sym.
+Definition q0 := (Ctx.q0,R).
+Definition s0 := @nil Ctx.Sym.
+Definition q_eqb := prod_eqb Ctx.q_eqb dir_eqb.
+Definition sym_eqb := list_eqb Ctx.sym_eqb.
+Lemma q_eqb_spec a b: Bool.reflect (a = b) (q_eqb a b).
+Proof.
+  intros.
+  apply prod_eqb_spec.
+  - apply Ctx.q_eqb_spec.
+  - apply dir_eqb_spec.
+Qed.
+Lemma sym_eqb_spec a b: Bool.reflect (a = b) (sym_eqb a b).
+Proof.
+  intros.
+  apply list_eqb_spec.
+  apply Ctx.sym_eqb_spec.
+Qed.
+Import HashConcat.
+Definition q_hash '(q,d) := Ctx.q_hash q ## dir_hash d.
+Definition sym_hash ls := list_hash Ctx.sym_hash ls.
+End BlockTMCtx.
+
+Module BlockTMFromDHTM(Ctx:Ctx).
+Module BlockTMCtx := BlockTMCtx Ctx.
+Module BlockTM := DHTM BlockTMCtx.
+Module DHTM := DHTM Ctx.
+
+Lemma repeat_const {A} (a:A) n:
+  repeat a n *> const a = const a.
+Proof.
+  induction n.
+  - reflexivity.
+  - cbn.
+    rewrite IHn,<-const_unfold.
+    reflexivity.
+Qed.
+
+Lemma const_unfold' {A} (a:A) h t:
+  h >> t = const a <->
+  (h = a /\ t = const a).
+Proof.
+  split.
+  - intros H.
+    rewrite const_unfold in H.
+    inverts H. tauto.
+  - intros [H H0].
+    subst.
+    rewrite <-const_unfold.
+    tauto.
+Qed.
+
+Section BlockSize.
+Hypothesis block_size block_time_limit:nat.
+Hypothesis block_size_nonzero: block_size <> O.
+Hypothesis tm:DHTM.TM.
+
+Definition map_TM:BlockTM.TM :=
+fun '((s,sgn),ls) =>
+let ls :=
+match ls with
+| nil => List.repeat Ctx.s0 block_size
+| _ => ls
+end in
+match (DHTM.DH_cconfig_bounded_progress tm (nil,ls,s,sgn) block_time_limit) with
+| None => None
+| Some (l0,r0,s0,sgn0) =>
+  match r0 with
+  | nil => Some (l0,sgn0,(s0,sgn0))
+  | _ => None
+  end
+end.
+
+Inductive map_cconfig: BlockTM.DH_cconfig -> DHTM.DH_cconfig -> Prop :=
+| map_cconfig_intro l r s sgn:
+  Forall (fun x => length x = block_size) l ->
+  Forall (fun x => length x = block_size) r ->
+  map_cconfig (l,r,(s,sgn),sgn) (concat l,concat r,s,sgn)
+.
+
+Ltac simpl_Forall_hyp :=
+  repeat
+  (match goal with
+  | H: _ |- _ => (rewrite Forall_cons_iff in H; cbn in H; try lia) || fail
+  | H: _ /\ _ |- _ => destruct H
+  end).
+
+Lemma Str_app_inv {a1 a2}:
+  a1 *> const BlockTMCtx.s0 = a2 *> const BlockTMCtx.s0 ->
+  Forall (fun x => length x = block_size) a1 ->
+  Forall (fun x => length x = block_size) a2 ->
+  a1 = a2.
+Proof.
+  gen a2.
+  induction a1; cbn; intros [|h2 t2] H H1 H2.
+  - reflexivity.
+  - cbn in H.
+    symmetry in H.
+    rewrite const_unfold' in H.
+    destruct H as [H Ha].
+    subst h2.
+    simpl_Forall_hyp.
+  - cbn in H.
+    rewrite const_unfold' in H.
+    destruct H as [H Ha].
+    subst a.
+    simpl_Forall_hyp.
+  - inverts H. f_equal.
+    simpl_Forall_hyp.
+    eapply IHa1; eauto.
+Qed.
+
+Lemma map_step c1 c1' c2'':
+  BlockTM.step map_TM (BlockTM.DH_cconfig_to_config c1) c2'' ->
+  map_cconfig c1 c1' ->
+  exists c2,
+  c2'' = (BlockTM.DH_cconfig_to_config c2) /\
+  exists c2',
+  map_cconfig c2 c2' /\
+  DHTM.progress tm (DHTM.DH_cconfig_to_config c1') (DHTM.DH_cconfig_to_config c2').
+Proof.
+  intros Hs C1.
+  inverts C1.
+  cbn in Hs.
+  cbn.
+  unfold map_TM in Hs.
+  inverts Hs.
+  - destruct m as [|m0 m1].
+    + pose proof (DHTM.DH_cconfig_bounded_progress_spec tm ([], repeat Ctx.s0 block_size, s, sgn) block_time_limit).
+      destruct (DHTM.DH_cconfig_bounded_progress tm ([], repeat Ctx.s0 block_size, s, sgn) block_time_limit) as [[[[l2 r2] s2] sgn2]|];
+      try congruence.
+      destruct r2 as [|r2 r3]; try congruence.
+      inverts H6.
+
+      destruct r as [|r4 r5].
+      2: cbn in H3; inverts H3;
+      rewrite Forall_cons_iff in H0; cbn in H0; lia.
+      inverts H3.
+
+      rewrite const_unfold' in H4.
+      destruct H4 as [_ H4].
+      subst r0.
+
+      destruct H1 as [H1' H1].
+      cbn in H1'.
+      rewrite repeat_length in H1'.
+
+      repeat rewrite <-const_unfold.
+      eexists (m'::l0,nil,(s2,sgn),sgn).
+      cbn.
+      split. 1: reflexivity.
+      eexists (_,_,_,_).
+      split.
+      * applys_eq map_cconfig_intro.
+        -- apply Forall_cons; auto 1; lia.
+        -- auto.
+      * cbn. cbn in H1.
+        repeat rewrite Str_app_assoc.
+        destruct sgn.
+        -- applys_eq H1.
+          repeat f_equal.
+          rewrite repeat_const; reflexivity.
+        -- applys_eq H1.
+          repeat f_equal.
+          rewrite repeat_const; reflexivity.
+
+    + pose proof (DHTM.DH_cconfig_bounded_progress_spec tm ([], m0 :: m1, s, sgn) block_time_limit).
+      destruct (DHTM.DH_cconfig_bounded_progress tm ([], m0 :: m1, s, sgn) block_time_limit) as [[[[l2 r2] s2] sgn2]|];
+      try congruence.
+      destruct r2 as [|r2 r3]; try congruence.
+      inverts H6.
+
+      destruct H1 as [H1' H1].
+      cbn in H1'.
+
+      destruct r as [|r4 r5].
+      1: { cbn in H3.
+        rewrite const_unfold' in H3.
+        unfold BlockTMCtx.s0 in H3.
+        destruct H3.
+        congruence.
+      }
+      inverts H3.
+
+      simpl_Forall_hyp.
+      eexists (m'::l0,r5,(s2,sgn),sgn).
+      cbn.
+      split. 1: reflexivity.
+      eexists (_,_,_,_).
+      split.
+      * applys_eq map_cconfig_intro.
+        -- apply Forall_cons; auto 1; lia.
+        -- auto.
+      * cbn. cbn in H1.
+        repeat rewrite Str_app_assoc.
+        destruct sgn; apply H1.
+
+  - destruct m as [|m0 m1].
+    + pose proof (DHTM.DH_cconfig_bounded_progress_spec tm ([], repeat Ctx.s0 block_size, s, sgn) block_time_limit).
+      destruct (DHTM.DH_cconfig_bounded_progress tm  ([], repeat Ctx.s0 block_size, s, sgn) block_time_limit) as [[[[l2 r2] s2] sgn2]|];
+      try congruence.
+
+      destruct r2 as [|r2 r3]; try congruence.
+      inverts H6.
+
+      destruct H1 as [H1' H1].
+      cbn in H1'.
+      rewrite repeat_length in H1'.
+
+      destruct r as [|r4 r5].
+      2: cbn in H3; inverts H3; simpl_Forall_hyp.
+      cbn in H3; inverts H3.
+
+      rewrite const_unfold' in H4.
+      destruct H4 as [_ H4].
+      subst r0.
+
+      repeat rewrite <-const_unfold.
+      eexists (m'::nil,l0,(s2,dir_rev sgn),dir_rev sgn).
+      cbn.
+      split. 1: reflexivity.
+      eexists (_,_,_,_).
+      split.
+      * applys_eq map_cconfig_intro.
+        -- apply Forall_cons; auto 1; lia.
+        -- auto.
+      * cbn. cbn in H1.
+        repeat rewrite Str_app_assoc.
+        destruct sgn.
+        -- applys_eq H1.
+          repeat f_equal. cbn.
+          rewrite repeat_const; reflexivity.
+        -- applys_eq H1.
+          repeat f_equal. cbn.
+          rewrite repeat_const; reflexivity.
+
+    + pose proof (DHTM.DH_cconfig_bounded_progress_spec tm ([], m0 :: m1, s, sgn) block_time_limit).
+      destruct (DHTM.DH_cconfig_bounded_progress tm ([], m0 :: m1, s, sgn) block_time_limit) as [[[[l2 r2] s2] sgn2]|];
+      try congruence.
+      destruct r2 as [|r2 r3]; try congruence.
+      inverts H6.
+      destruct H1 as [H1' H1].
+      cbn in H1'.
+
+      destruct r as [|r4 r5].
+      1: { cbn in H3.
+        rewrite const_unfold' in H3.
+        unfold BlockTMCtx.s0 in H3.
+        destruct H3.
+        congruence.
+      }
+      inverts H3.
+
+      simpl_Forall_hyp.
+      eexists (m'::r5,l0,(s2,dir_rev sgn),dir_rev sgn).
+      cbn.
+      split. 1: reflexivity.
+      eexists (_,_,_,_).
+      split.
+      * applys_eq map_cconfig_intro.
+        -- apply Forall_cons; auto 1; lia.
+        -- auto.
+      * cbn. cbn in H1.
+        repeat rewrite Str_app_assoc.
+        destruct sgn; apply H1.
+Qed.
+
+Definition P c1'' := exists c1 c1',
+  map_cconfig c1 c1' /\
+  c1'' = (DHTM.DH_cconfig_to_config c1') /\
+  ~BlockTM.halts map_TM (BlockTM.DH_cconfig_to_config c1).
+
+Lemma map_nonhalt c1 c1':
+  ~BlockTM.halts' map_TM (BlockTM.DH_cconfig_to_config c1) ->
+  map_cconfig c1 c1' ->
+  ~DHTM.halts' tm (DHTM.DH_cconfig_to_config c1').
+Proof.
+  rewrite <-BlockTM.halts_halts'.
+  rewrite <-DHTM.halts_halts'.
+  intros H H0.
+  apply DHTM.progress_nonhalt with (P:=P).
+  - intros c'' Pc.
+    unfold P in Pc.
+    destruct Pc as [c [c' [H1 [H2 H3]]]].
+    pose proof (BlockTM.DH_cconfig_step_spec map_TM c).
+    destruct (BlockTM.DH_cconfig_step map_TM c) as [c2|] eqn:E.
+    * epose proof (map_step _ _ _ H4 H1) as H5.
+      destruct H5 as [c2_ [H5 [c2' [H6 H7]]]].
+      exists (DHTM.DH_cconfig_to_config c2').
+      subst c''.
+      split; auto 1.
+      unfold P.
+      eexists _,_.
+      split. 1: apply H6.
+      split. 1: reflexivity.
+      intros [n0 [c3 Hh]].
+      apply H3.
+      exists (S n0),c3.
+      split. 2: tauto.
+      econstructor; eauto.
+      rewrite H5.
+      apply Hh.
+    * assert False. {
+        apply H3.
+        eexists _,_.
+        split. 2: apply H4.
+        constructor.
+      }
+      tauto.
+  - unfold P.
+    eexists _,_.
+    split. 1: apply H0.
+    split. 1: reflexivity.
+    apply H.
+Qed.
+
+Fixpoint inv_map_cside(ls:list Ctx.Sym)(n:nat):(BlockTMCtx.Sym)*(list BlockTMCtx.Sym) :=
+match ls with
+| nil => (List.repeat Ctx.s0 n,nil)
+| h::t =>
+  match n with
+  | O =>
+    let (a,b):=inv_map_cside t (Nat.pred block_size) in (nil,(h::a)::b)
+  | S n =>
+    let (a,b):=inv_map_cside t n in (h::a,b)
+  end
+end.
+
+Definition inv_map_cconfig(x:DHTM.DH_cconfig):BlockTM.DH_cconfig :=
+let '(l,r,s,sgn):=x in
+let (l0,l1):=inv_map_cside l block_size in
+let (r0,r1):=inv_map_cside r block_size in
+(l0::l1,r0::r1,(s,sgn),sgn).
+
+Lemma inv_map_cside_spec' l n s0 l0:
+  inv_map_cside l n = (s0, l0) ->
+  (Forall (fun x : list Ctx.Sym => length x = block_size) l0 /\
+  length s0 = n /\
+  s0 *> concat l0 *> const Ctx.s0 = l *> const Ctx.s0).
+Proof.
+  gen n s0 l0.
+  induction l; intros.
+  - inverts H.
+    repeat split. 1: auto.
+    1: apply repeat_length.
+    cbn.
+    rewrite repeat_const.
+    reflexivity.
+  - cbn in H.
+    destruct n as [|n].
+    + destruct (inv_map_cside l (Nat.pred block_size)) eqn:E1.
+      inverts H.
+      specialize (IHl _ _ _ E1).
+      cbn.
+      repeat rewrite Str_app_assoc.
+      repeat split.
+      * apply Forall_cons.
+        -- cbn. lia.
+        -- apply IHl.
+      * f_equal. apply IHl.
+    + destruct (inv_map_cside l n) eqn:E1.
+      inverts H.
+      specialize (IHl _ _ _ E1).
+      cbn.
+      repeat split.
+      * apply IHl.
+      * lia.
+      * f_equal. apply IHl.
+Qed.
+
+Lemma inv_map_cside_spec l s0 l0:
+  inv_map_cside l block_size = (s0, l0) ->
+  (Forall (fun x : list Ctx.Sym => length x = block_size) (s0 :: l0) /\
+  s0 *> concat l0 *> const Ctx.s0 = l *> const Ctx.s0).
+Proof.
+  intros H.
+  pose proof (inv_map_cside_spec' _ _ _ _ H).
+  split.
+  - apply Forall_cons; tauto.
+  - tauto.
+Qed.
+
+Lemma inv_map_cconfig_spec x:
+  exists x', map_cconfig (inv_map_cconfig x) x' /\ DHTM.DH_cconfig_to_config x' = DHTM.DH_cconfig_to_config x.
+Proof.
+  destruct x as [[[l r] s] sgn].
+  cbn.
+  destruct (inv_map_cside l block_size) eqn:El.
+  destruct (inv_map_cside r block_size) eqn:Er.
+  pose proof (inv_map_cside_spec _ _ _ El) as Hl.
+  pose proof (inv_map_cside_spec _ _ _ Er) as Hr.
+  cbn.
+  eexists.
+  split.
+  - econstructor.
+    + apply Hl.
+    + apply Hr.
+  - cbn.
+    repeat rewrite Str_app_assoc.
+    do 3 f_equal.
+    + apply Hl.
+    + apply Hr.
+Qed.
+
+Lemma inv_map_nonhalt c1':
+  ~BlockTM.halts' map_TM (BlockTM.DH_cconfig_to_config (inv_map_cconfig c1')) ->
+  ~DHTM.halts' tm (DHTM.DH_cconfig_to_config c1').
+Proof.
+  destruct (inv_map_cconfig_spec c1') as [c1 [H H0]].
+  intros H1.
+  rewrite <-H0.
+  apply (map_nonhalt _ _ H1 H).
+Qed.
+
+End BlockSize.
+
+End BlockTMFromDHTM.
+
+
+
+Module Type NonEmptyHashableType(HT:HashableType).
+Export HT.
+Parameter k0: K.
+End NonEmptyHashableType.
+
+Module TapeHistoryTMCtx(Ctx:Ctx)(HT:HashableType)(th:NonEmptyHashableType HT) <: Ctx.
+Export th.
+Definition Q:Type := Ctx.Q.
+Definition Sym:Type := Ctx.Sym*K.
+Definition q0 := Ctx.q0.
+Definition s0 := (Ctx.s0,k0).
+Definition q_eqb := Ctx.q_eqb.
+Definition sym_eqb := prod_eqb Ctx.sym_eqb K_eq.
+Definition q_eqb_spec := Ctx.q_eqb_spec.
+Lemma sym_eqb_spec a b: Bool.reflect (a = b) (sym_eqb a b).
+Proof.
+  intros.
+  apply prod_eqb_spec.
+  - apply Ctx.sym_eqb_spec.
+  - apply K_eq_spec.
+Qed.
+Import HashConcat.
+Definition q_hash := Ctx.q_hash.
+Definition sym_hash '(s,h) := (Ctx.sym_hash s) ## (K_hash h).
+End TapeHistoryTMCtx.
+
+
+Module TapeHistoryTMFromDHTM(Ctx:Ctx)(HT:HashableType)(th:NonEmptyHashableType HT).
+
+Module TapeHistoryTMCtx := TapeHistoryTMCtx Ctx HT th.
+Module TapeHistoryTM := DHTM TapeHistoryTMCtx.
+Module DHTM := DHTM Ctx.
+
+Section map_ctx.
+
+Hypothesis tm:DHTM.TM.
+Hypothesis history_upd:Ctx.Q->Ctx.Sym->HT.K->HT.K.
+Definition map_TM:TapeHistoryTM.TM :=
+fun '(s,(m,k)) =>
+match tm (s,m) with
+| None => None
+| Some (m',sgn',s') =>
+  Some ((m',history_upd s m k),sgn',s')
+end.
+
+Definition map_cside(x:list TapeHistoryTMCtx.Sym):list Ctx.Sym :=
+List.map fst x.
+
+Definition inv_map_cside(x:list Ctx.Sym):list TapeHistoryTMCtx.Sym :=
+List.map (fun a => (a,th.k0)) x.
+
+Definition map_cconfig(x:TapeHistoryTM.DH_cconfig):DHTM.DH_cconfig :=
+let '(l,r,s,sgn):=x in
+(map_cside l,map_cside r,s,sgn).
+
+Definition inv_map_cconfig(x:DHTM.DH_cconfig):TapeHistoryTM.DH_cconfig :=
+let '(l,r,s,sgn):=x in
+(inv_map_cside l,inv_map_cside r,s,sgn).
+
+Lemma map_step c1 c2'':
+  TapeHistoryTM.step map_TM (TapeHistoryTM.DH_cconfig_to_config c1) c2'' ->
+  exists c2,
+  c2'' = (TapeHistoryTM.DH_cconfig_to_config c2) /\
+  DHTM.step tm (DHTM.DH_cconfig_to_config (map_cconfig c1)) (DHTM.DH_cconfig_to_config (map_cconfig c2)).
+Proof.
+  intros H.
+  destruct c1 as [[[l1 r1] s1] sgn1]; cbn in H.
+  inverts H.
+  - unfold map_TM in H5.
+    destruct m as [m k].
+    destruct r1 as [|[m1 k1] r1].
+    + cbn in H2.
+      rewrite const_unfold in H2.
+      inverts H2. cbn.
+      eexists (m'::l1,nil,s',sgn1); cbn.
+      split. 1: reflexivity.
+      unfold map_cside.
+      applys_eq DHTM.step_through.
+      1: rewrite <-const_unfold; reflexivity.
+      destruct (tm (s1, Ctx.s0)) as [[[m'' sgn'] s'']|] eqn:E; try congruence.
+      unfold TapeHistoryTMCtx.Q in E.
+      rewrite E.
+      inverts H5. reflexivity.
+    + cbn in H2.
+      inverts H2. cbn.
+      eexists (m'::l1,r1,_,_); cbn.
+      split. 1: reflexivity.
+      unfold map_cside.
+      applys_eq DHTM.step_through.
+      destruct (tm (s1, m1)) as [[[m'' sgn'] s'']|] eqn:E; try congruence.
+      unfold TapeHistoryTMCtx.Q in E.
+      rewrite E.
+      inverts H5. reflexivity.
+  - unfold map_TM in H5.
+    destruct m as [m k].
+    destruct r1 as [|[m1 k1] r1].
+    + cbn in H2.
+      rewrite const_unfold in H2.
+      inverts H2. cbn.
+      eexists (m'::nil,l1,_,_); cbn.
+      split. 1: reflexivity.
+      unfold map_cside.
+      applys_eq DHTM.step_back.
+      1: rewrite <-const_unfold; reflexivity.
+      destruct (tm (s1, Ctx.s0)) as [[[m'' sgn'] s'']|] eqn:E; try congruence.
+      unfold TapeHistoryTMCtx.Q in E.
+      rewrite E.
+      inverts H5. reflexivity.
+    + cbn in H2.
+      inverts H2. cbn.
+      eexists (m'::r1,l1,_,_); cbn.
+      split. 1: reflexivity.
+      unfold map_cside.
+      applys_eq DHTM.step_back.
+      destruct (tm (s1, m1)) as [[[m'' sgn'] s'']|] eqn:E; try congruence.
+      unfold TapeHistoryTMCtx.Q in E.
+      rewrite E.
+      inverts H5. reflexivity.
+Qed.
+
+Lemma map_multistep n c1 c2'':
+  TapeHistoryTM.multistep map_TM n (TapeHistoryTM.DH_cconfig_to_config c1) c2'' ->
+  exists c2,
+  c2'' = (TapeHistoryTM.DH_cconfig_to_config c2) /\
+  DHTM.multistep tm n (DHTM.DH_cconfig_to_config (map_cconfig c1)) (DHTM.DH_cconfig_to_config (map_cconfig c2)).
+Proof.
+  gen c1 c2''.
+  induction n; intros.
+  - exists c1.
+    inverts H.
+    split.
+    1: reflexivity.
+    constructor.
+  - inverts H.
+    destruct (map_step c1 c' H1) as [c [H3 H4]].
+    subst c'.
+    destruct (IHn c c2'' H2) as [c2 [H5 H6]].
+    eexists.
+    split. 1: apply H5.
+    econstructor; eauto.
+Qed.
+
+Lemma map_nonhalt c1:
+  ~TapeHistoryTM.halts map_TM (TapeHistoryTM.DH_cconfig_to_config c1) ->
+  ~DHTM.halts tm (DHTM.DH_cconfig_to_config (map_cconfig c1)).
+Proof.
+  rewrite TapeHistoryTM.nonhalt_iff.
+  rewrite DHTM.nonhalt_iff.
+  intros H n.
+  specialize (H n).
+  destruct H as [c' H].
+  destruct (map_multistep _ _ _ H) as [c2 [H0 H1]].
+  eexists; eauto.
+Qed.
+
+Lemma inv_map_cside_spec ls:
+  map_cside (inv_map_cside ls) = ls.
+Proof.
+  unfold map_cside,inv_map_cside.
+  induction ls; cbn.
+  1: reflexivity.
+  rewrite IHls.
+  reflexivity.
+Qed.
+
+Lemma inv_map_cconfig_spec c:
+  map_cconfig (inv_map_cconfig c) = c.
+Proof.
+  destruct c as [[[l r] s] sgn]; cbn.
+  do 2 rewrite inv_map_cside_spec.
+  reflexivity.
+Qed.
+
+Lemma inv_map_nonhalt c1:
+  ~TapeHistoryTM.halts' map_TM (TapeHistoryTM.DH_cconfig_to_config (inv_map_cconfig c1)) ->
+  ~DHTM.halts' tm (DHTM.DH_cconfig_to_config c1).
+Proof.
+  rewrite <-TapeHistoryTM.halts_halts'.
+  rewrite <-DHTM.halts_halts'.
+  intros H.
+  applys_eq (map_nonhalt _ H).
+  rewrite inv_map_cconfig_spec.
+  reflexivity.
+Qed.
+
+End map_ctx.
+
+End TapeHistoryTMFromDHTM.
+
+Fixpoint remove_nth{A}(f:A->bool)(n:nat)(ls:list A):list A :=
+match ls with
+| nil => nil
+| h::t =>
+  if f h then
+    match n with
+    | O => t
+    | S n0 => h::remove_nth f n0 t
+    end
+  else h::remove_nth f n t
+end.
+
+Fixpoint upd_skipn{A}(n:nat)(f:list A->list A)(ls:list A) :=
+match n with
+| O => f ls
+| S n0 =>
+  match ls with
+  | nil => nil
+  | h::ls0 => h::upd_skipn n0 f ls0
+  end
+end.
+
+Definition upd_LRU{A}(n LRU_n:nat)(A_eqb:A->A->bool)(ls:list A) :=
+match ls with
+| nil => nil
+| h::ls0 => firstn n (h::(remove_nth (A_eqb h) LRU_n ls0))
+end.
+
+Definition upd_skipn_LRU{A}(n1 n2 LRU_n:nat)(A_eqb:A->A->bool)(ls:list A) :=
+upd_skipn n1 (fun ls => upd_LRU n2 LRU_n A_eqb ls) ls.
+
+
+
+
+Module RWL_mod(Ctx:Ctx).
+
+Module SymHash := SymHash Ctx.
+Module Int2Hash := ProdHash Uint63_K Uint63_K.
+Module Int3Hash := ProdHash Int2Hash Uint63_K.
+Module ListInt3Hash := ListHash Int3Hash.
+
+Fixpoint limit_length{A}(len1 len2:nat)(ls:list A):list A :=
+match len1 with
+| O => if List.length ls <=? len2 then ls else (List.tl ls)
+| S len1' =>
+  match ls with
+  | nil => nil
+  | h::t => h::(limit_length len1' len2 t)
+  end
+end.
+
+Module CTLCtx <: CTLCtx ListInt3Hash Ctx.
+Module SymIdAlloc := IdAlloc SymHash.
+Record config := {
+  mnc: Uint63.int;
+  mod_: Uint63.int;
+  len1: nat;
+  len2: nat;
+  maxS: Uint63.int;
+  is_s0: Ctx.Sym->bool;
+}.
+Definition config_t:Type := config.
+Definition global_state_t:Type := config_t*SymIdAlloc.id_alloc_t.
+Definition global_state_init cfg := (cfg,SymIdAlloc.id_alloc_make cfg.(maxS)).
+Definition dfa_state_0 := @nil Int3Hash.K.
+
+Definition dfa_trans(x:ListInt3Hash.K)(y0:Ctx.Sym)(d:dir)(gs:global_state_t):ListInt3Hash.K*global_state_t :=
+let (cfg,gs):=gs in
+match SymIdAlloc.get_or_alloc_id y0 gs with
+| None => (nil,(cfg,gs))
+| Some (y,gs) =>
+  (match x with
+  | nil => if cfg.(is_s0) y0 then nil else (y,int1,int1)::nil
+  | (x0,n,m)::x1 =>
+    let x' :=
+    (if Uint63.eqb x0 y then
+      (x0,
+       if Uint63.ltb n cfg.(mnc) then Uint63.add n int1 else cfg.(mnc),
+       Uint63.mod (Uint63.add m int1) cfg.(mod_))::
+       x1
+    else (y,int1,int1)::x)
+    in limit_length cfg.(len1) cfg.(len2) x'
+  end,(cfg,gs))
+end.
+End CTLCtx.
+
+End RWL_mod.
+
+
+
+Module CPS_LRU(Ctx:Ctx).
+
+Module SymHash := SymHash Ctx.
+Module ListIntHash := ListHash Uint63_K.
+Module List2IntHash := ProdHash ListIntHash ListIntHash.
+
+Module CTLCtx <: CTLCtx List2IntHash Ctx.
+Module SymIdAlloc := IdAlloc SymHash.
+Record config := {
+  len1: nat;
+  len2: nat;
+  len3: nat;
+  LRU_n: nat;
+  maxS: Uint63.int;
+  is_s0: Ctx.Sym->bool;
+}.
+
+Definition config_t:Type := config.
+Definition global_state_t:Type := config_t*SymIdAlloc.id_alloc_t.
+Definition global_state_init cfg := (cfg,SymIdAlloc.id_alloc_make cfg.(maxS)).
+Definition dfa_state_0:List2IntHash.K := (nil,nil).
+
+Definition is_nil{A}(ls:list A):bool :=
+match ls with
+| nil => true
+| _ => false
+end.
+
+Definition dfa_trans(x:List2IntHash.K)(y0:Ctx.Sym)(d:dir)(gs:global_state_t):List2IntHash.K*global_state_t :=
+let (cfg,gs):=gs in
+match SymIdAlloc.get_or_alloc_id y0 gs with
+| None => ((nil,nil),(cfg,gs))
+| Some (y,gs) =>
+  let '(x12,x3):=x in
+  if is_nil x12 && is_nil x3 && cfg.(is_s0) y0 then ((nil,nil),(cfg,gs))
+  else
+  let x' :=
+  (if length x3 <? cfg.(len3) then
+    (x12,y::x3)
+  else
+    (upd_skipn_LRU cfg.(len1) cfg.(len2) cfg.(LRU_n) Uint63.eqb (y::x12),x3)
+  ) in
+  (x',(cfg,gs))
+end.
+
+End CTLCtx.
+End CPS_LRU.
+
+
+Module NGramCPS(Ctx:Ctx).
+
+Module SymHash := SymHash Ctx.
+Module ListIntHash := ListHash Uint63_K.
+
+Module CTLCtx <: CTLCtx ListIntHash Ctx.
+Module SymIdAlloc := IdAlloc SymHash.
+Record config := {
+  len: nat;
+  maxS: Uint63.int;
+}.
+
+Definition config_t:Type := config.
+Definition global_state_t:Type := config_t*SymIdAlloc.id_alloc_t.
+Definition global_state_init cfg := (cfg,SymIdAlloc.id_alloc_make cfg.(maxS)).
+Definition dfa_state_0:ListIntHash.K := (nil).
+
+Definition dfa_trans(x:ListIntHash.K)(y:Ctx.Sym)(d:dir)(gs:global_state_t):ListIntHash.K*global_state_t :=
+let (cfg,gs):=gs in
+match SymIdAlloc.get_or_alloc_id y gs with
+| None => ((nil),(cfg,gs))
+| Some (y,gs) =>
+  (firstn cfg.(len) (y::x),(cfg,gs))
+end.
+
+End CTLCtx.
+
+End NGramCPS.
+
+
+Module TapeHistoryImpl(Ctx:Ctx).
+Module QHash := QHash Ctx.
+Module SymHash := SymHash Ctx.
+Module QSymHash := ProdHash QHash SymHash.
+Module ListSymHash := ListHash SymHash.
+Module ListQSymHash := ListHash QSymHash.
+
+Module ListSymNonEmptyHash <: NonEmptyHashableType ListSymHash.
+Definition k0 := @nil (Ctx.Sym).
+End ListSymNonEmptyHash.
+
+Module ListQSymNonEmptyHash <: NonEmptyHashableType ListQSymHash.
+Definition k0 := @nil (Ctx.Q*Ctx.Sym).
+End ListQSymNonEmptyHash.
+
+Module ListSymTapeHistoryTMFromDHTM := TapeHistoryTMFromDHTM Ctx ListSymHash ListSymNonEmptyHash.
+Module ListQSymTapeHistoryTMFromDHTM := TapeHistoryTMFromDHTM Ctx ListQSymHash ListQSymNonEmptyHash.
+
+Definition Sym_history_upd(len1 len2 LRU_n:nat)(s:Ctx.Q)(m:Ctx.Sym)(ls:ListSymHash.K): ListSymHash.K :=
+upd_skipn_LRU len1 len2 LRU_n SymHash.K_eq (m::ls).
+
+Definition QSym_history_upd(len1 len2 LRU_n:nat)(s:Ctx.Q)(m:Ctx.Sym)(ls:ListQSymHash.K): ListQSymHash.K :=
+upd_skipn_LRU len1 len2 LRU_n QSymHash.K_eq ((s,m)::ls).
+
+End TapeHistoryImpl.
+
+Definition N_to_int x := Uint63.of_Z (Z.of_N x).
+
+Module CTLDecider(Ctx:TM.Ctx).
+
+Module DHTMFromTM := DHTMFromTM Ctx.
+Module BlockTMFromDHTM := BlockTMFromDHTM DHTMFromTM.TMCtx.
+Module TapeHistoryImpl := TapeHistoryImpl DHTMFromTM.TMCtx.
+
+Module Ctx_RWL_mod := RWL_mod BlockTMFromDHTM.BlockTMCtx.
+Module CTL_RWL_mod := CTL Ctx_RWL_mod.ListInt3Hash BlockTMFromDHTM.BlockTMCtx Ctx_RWL_mod.CTLCtx.
+
+Module Ctx_CPS_LRU := CPS_LRU BlockTMFromDHTM.BlockTMCtx.
+Module CTL_CPS_LRU := CTL Ctx_CPS_LRU.List2IntHash BlockTMFromDHTM.BlockTMCtx Ctx_CPS_LRU.CTLCtx.
+
+Module Ctx_NG_Sym := NGramCPS TapeHistoryImpl.ListSymTapeHistoryTMFromDHTM.TapeHistoryTMCtx.
+Module Ctx_NG_QSym := NGramCPS TapeHistoryImpl.ListQSymTapeHistoryTMFromDHTM.TapeHistoryTMCtx.
+Module CTL_NG_Sym := CTL
+  Ctx_NG_Sym.ListIntHash
+  TapeHistoryImpl.ListSymTapeHistoryTMFromDHTM.TapeHistoryTMCtx
+  Ctx_NG_Sym.CTLCtx.
+Module CTL_NG_QSym := CTL
+  Ctx_NG_QSym.ListIntHash
+  TapeHistoryImpl.ListQSymTapeHistoryTMFromDHTM.TapeHistoryTMCtx
+  Ctx_NG_QSym.CTLCtx.
+
+Inductive DeciderParameter :=
+| RWL_mod(simT maxT maxS bsz bmaxT mnc mod_ len1 len2:N)
+| CPS_LRU(simT maxT maxS bsz bmaxT len1 len2 len3 LRU_n:N)
+| NG(simT maxT maxS NG_n len1 len2 LRU_n:N)(asth:bool)
+.
+
+Section tm_ctx.
+Hypothesis tm:DHTMFromTM.TM.TM.
+Hypothesis arg:DeciderParameter.
+Definition decide_nonhalt:bool :=
+match arg with
+| RWL_mod simT maxT maxS bsz bmaxT mnc mod_ len1 len2 =>
+  match DHTMFromTM.DHTM.DH_cconfig_steps tm DHTMFromTM.DHTM.cc0 simT with
+  | inl c =>
+    let bsz := N.max 1 bsz in
+    let tm1 := (BlockTMFromDHTM.map_TM (N.to_nat bsz) (N.to_nat bmaxT) tm) in
+    let c1 := (BlockTMFromDHTM.inv_map_cconfig (N.to_nat bsz) c) in
+    let cfg :=
+      {|
+        Ctx_RWL_mod.CTLCtx.mnc := N_to_int mnc;
+        Ctx_RWL_mod.CTLCtx.mod_ := N_to_int mod_;
+        Ctx_RWL_mod.CTLCtx.len1 := N.to_nat len1;
+        Ctx_RWL_mod.CTLCtx.len2 := N.to_nat len2;
+        Ctx_RWL_mod.CTLCtx.maxS := N_to_int maxS;
+        Ctx_RWL_mod.CTLCtx.is_s0 := fun ls => forallb (DHTMFromTM.TMCtx.sym_eqb DHTMFromTM.TMCtx.s0) ls;
+      |} in
+    (CTL_RWL_mod.CTL_decide_nonhalt tm1 c1 cfg (N_to_int maxS) (maxT*100))
+  | inr c => false
+  end
+| CPS_LRU simT maxT maxS bsz bmaxT len1 len2 len3 LRU_n =>
+  match DHTMFromTM.DHTM.DH_cconfig_steps tm DHTMFromTM.DHTM.cc0 simT with
+  | inl c =>
+    let bsz := N.max 1 bsz in
+    let tm1 := (BlockTMFromDHTM.map_TM (N.to_nat bsz) (N.to_nat bmaxT) tm) in
+    let c1 := (BlockTMFromDHTM.inv_map_cconfig (N.to_nat bsz) c) in
+    let cfg := 
+      {|
+        Ctx_CPS_LRU.CTLCtx.len1 := N.to_nat len1;
+        Ctx_CPS_LRU.CTLCtx.len2 := N.to_nat len2;
+        Ctx_CPS_LRU.CTLCtx.len3 := N.to_nat len3;
+        Ctx_CPS_LRU.CTLCtx.LRU_n := N.to_nat LRU_n;
+        Ctx_CPS_LRU.CTLCtx.maxS := N_to_int maxS;
+        Ctx_CPS_LRU.CTLCtx.is_s0 := fun ls => forallb (DHTMFromTM.TMCtx.sym_eqb DHTMFromTM.TMCtx.s0) ls;
+      |} in
+    (CTL_CPS_LRU.CTL_decide_nonhalt tm1 c1 cfg (N_to_int maxS) (maxT*100))
+  | inr c => false
+  end
+| NG simT maxT maxS NG_n len1 len2 LRU_n asth =>
+  match DHTMFromTM.DHTM.DH_cconfig_steps tm DHTMFromTM.DHTM.cc0 simT with
+  | inl c =>
+    let '(len1,len2,LRU_n):=(N.to_nat len1,N.to_nat len2,N.to_nat LRU_n) in
+    if asth then
+      let upd := TapeHistoryImpl.QSym_history_upd len1 len2 LRU_n in
+      let tm1 := TapeHistoryImpl.ListQSymTapeHistoryTMFromDHTM.map_TM tm upd in
+      let c1 := TapeHistoryImpl.ListQSymTapeHistoryTMFromDHTM.inv_map_cconfig c in
+      let cfg :=
+        {|
+          Ctx_NG_QSym.CTLCtx.len := N.to_nat NG_n;
+          Ctx_NG_QSym.CTLCtx.maxS := N_to_int maxS;
+        |} in
+      (CTL_NG_QSym.CTL_decide_nonhalt tm1 c1 cfg (N_to_int maxS) (maxT*100))
+    else
+      let upd := TapeHistoryImpl.Sym_history_upd len1 len2 LRU_n in
+      let tm1 := TapeHistoryImpl.ListSymTapeHistoryTMFromDHTM.map_TM tm upd in
+      let c1 := TapeHistoryImpl.ListSymTapeHistoryTMFromDHTM.inv_map_cconfig c in
+      let cfg :=
+        {|
+          Ctx_NG_Sym.CTLCtx.len := N.to_nat NG_n;
+          Ctx_NG_Sym.CTLCtx.maxS := N_to_int maxS;
+        |} in
+      (CTL_NG_Sym.CTL_decide_nonhalt tm1 c1 cfg (N_to_int maxS) maxT)
+  | inr c => false
+  end
+end.
+
+Lemma decide_nonhalt_spec:
+  decide_nonhalt = true ->
+  ~DHTMFromTM.TM.halts' tm DHTMFromTM.TM.c0.
+Proof.
+  unfold decide_nonhalt.
+  intros H.
+  destruct arg.
+  - apply DHTMFromTM.map_nonhalt.
+    pose proof (DHTMFromTM.DHTM.DH_cconfig_steps_spec tm DHTMFromTM.DHTM.cc0 simT) as H0.
+    destruct (DHTMFromTM.DHTM.DH_cconfig_steps tm DHTMFromTM.DHTM.cc0 simT); try congruence.
+    rewrite <-DHTMFromTM.DHTM.halts_halts'.
+    eapply DHTMFromTM.DHTM.evstep_nonhalt; eauto. clear H0.
+    epose proof (CTL_RWL_mod.CTL_decide_nonhalt_spec _ _ _ _ _ H) as H1.
+    rewrite DHTMFromTM.DHTM.halts_halts'.
+    rewrite CTL_RWL_mod.TM.halts_halts' in H1.
+    eapply BlockTMFromDHTM.inv_map_nonhalt.
+    2: apply H1.
+    lia.
+  - apply DHTMFromTM.map_nonhalt.
+    pose proof (DHTMFromTM.DHTM.DH_cconfig_steps_spec tm DHTMFromTM.DHTM.cc0 simT) as H0.
+    destruct (DHTMFromTM.DHTM.DH_cconfig_steps tm DHTMFromTM.DHTM.cc0 simT); try congruence.
+    rewrite <-DHTMFromTM.DHTM.halts_halts'.
+    eapply DHTMFromTM.DHTM.evstep_nonhalt; eauto. clear H0.
+    epose proof (CTL_CPS_LRU.CTL_decide_nonhalt_spec _ _ _ _ _ H) as H1.
+    rewrite DHTMFromTM.DHTM.halts_halts'.
+    rewrite CTL_CPS_LRU.TM.halts_halts' in H1.
+    eapply BlockTMFromDHTM.inv_map_nonhalt.
+    2: apply H1.
+    lia.
+  - apply DHTMFromTM.map_nonhalt.
+    pose proof (DHTMFromTM.DHTM.DH_cconfig_steps_spec tm DHTMFromTM.DHTM.cc0 simT) as H0.
+    destruct (DHTMFromTM.DHTM.DH_cconfig_steps tm DHTMFromTM.DHTM.cc0 simT); try congruence.
+    rewrite <-DHTMFromTM.DHTM.halts_halts'.
+    eapply DHTMFromTM.DHTM.evstep_nonhalt; eauto. clear H0.
+    destruct asth.
+    + epose proof (CTL_NG_QSym.CTL_decide_nonhalt_spec _ _ _ _ _ H) as H1.
+      rewrite DHTMFromTM.DHTM.halts_halts'.
+      rewrite CTL_NG_QSym.TM.halts_halts' in H1.
+      eapply TapeHistoryImpl.ListQSymTapeHistoryTMFromDHTM.inv_map_nonhalt.
+      apply H1.
+    + epose proof (CTL_NG_Sym.CTL_decide_nonhalt_spec _ _ _ _ _ H) as H1.
+      rewrite DHTMFromTM.DHTM.halts_halts'.
+      rewrite CTL_NG_Sym.TM.halts_halts' in H1.
+      eapply TapeHistoryImpl.ListSymTapeHistoryTMFromDHTM.inv_map_nonhalt.
+      apply H1.
+Qed.
+
+End tm_ctx.
+
+End CTLDecider.
+
+
+
