verify/CTL62.v
@@ -1,0 +1,20 @@
+Require Export String.
+Require Export NArith.
+From BusyCoq Require Export Individual62.
+From BusyCoq Require Export CTL.
+
+Module CTLDecider62 := CTLDecider BB62.
+Export CTLDecider62.
+
+Open Scope N.
+Open Scope string.
+
+Ltac solve_cert cert :=
+  match goal with
+  | |- ~halts (TM_from_str ?tm) c0 =>
+    idtac tm;
+    rewrite halts_halts';
+    eapply (decide_nonhalt_spec _ cert);
+    vm_cast_no_check (eq_refl true)
+  end.
+
