verify/DHTM.v
@@ -1,0 +1,586 @@
+From Coq Require Import Bool.
+From Coq Require Import Lists.List. Export ListNotations.
+From Coq Require Import Lists.Streams.
+From Coq Require Import NArith.
+From Coq Require Import PeanoNat.
+From Coq Require Import Lia.
+From BusyCoq Require Export TM.
+From BusyCoq Require Import HashTable.
+
+Module Type Ctx.
+  (** the type of states [Q]; *)
+  Parameter Q : Type.
+  (** the type of tape symbols [Sym]; *)
+  Parameter Sym : Type.
+  (** the starting state [q0]; *)
+  Parameter q0 : Q.
+  (** and the blank symbol [s0]. *)
+  Parameter s0 : Sym.
+
+  Parameter q_eqb : Q->Q->bool.
+  Parameter sym_eqb : Sym->Sym->bool.
+  Parameter q_eqb_spec : forall a b:Q, Bool.reflect (a=b) (q_eqb a b).
+  Parameter sym_eqb_spec : forall a b:Sym, Bool.reflect (a=b) (sym_eqb a b).
+  Parameter q_hash : Q->HashConcat.hash_t.
+  Parameter sym_hash : Sym->HashConcat.hash_t.
+End Ctx.
+
+Module QHash(Ctx:Ctx) <: HashableType.
+Import Ctx.
+Definition K := Q.
+Definition K_eq := q_eqb.
+Definition K_eq_spec := q_eqb_spec.
+Definition K_hash := q_hash.
+End QHash.
+
+Module SymHash(Ctx:Ctx) <: HashableType.
+Import Ctx.
+Definition K := Sym.
+Definition K_eq := sym_eqb.
+Definition K_eq_spec := sym_eqb_spec.
+Definition K_hash := sym_hash.
+End SymHash.
+
+
+Module DHTM (Ctx : Ctx).
+  Export Ctx.
+
+Definition TM : Type := Q * Sym -> option (Sym * dir * Q).
+
+Notation side := (Stream Sym).
+Notation DH_config := (side * side * Q * dir)%type.
+
+Reserved Notation "c -[ tm ]-> c'" (at level 40).
+
+Inductive step (tm:TM): DH_config->DH_config->Prop :=
+| step_through l m m' r s s' sgn:
+  tm (s,m) = Some (m',sgn,s') ->
+  step tm (l,m >> r,s,sgn) (m' >> l,r,s',sgn)
+| step_back l m m' r s s' sgn:
+  tm (s,m) = Some (m',dir_rev sgn,s') ->
+  step tm (l,m >> r,s,sgn) (m' >> r,l,s',dir_rev sgn)
+  where "c -[ tm ]-> c'" := (step tm c c').
+
+#[export] Hint Constructors step : core.
+
+
+Reserved Notation "c -[ tm ]->> n / c'" (at level 40, n at next level).
+
+Inductive multistep (tm : TM) : nat -> DH_config -> DH_config -> Prop :=
+  | multistep_0 c : c -[ tm ]->> 0 / c
+  | multistep_S n c c' c'' :
+    c  -[ tm ]->  c' ->
+    c' -[ tm ]->> n / c'' ->
+    c  -[ tm ]->> S n / c''
+
+  where "c -[ tm ]->> n / c'" := (multistep tm n c c').
+
+#[export] Hint Constructors multistep : core.
+
+
+Reserved Notation "c -[ tm ]->* c'" (at level 40).
+
+Inductive evstep (tm : TM) : DH_config -> DH_config -> Prop :=
+  | evstep_refl c : c -[ tm ]->* c
+  | evstep_step c c' c'' :
+    c  -[ tm ]->  c'  ->
+    c' -[ tm ]->* c'' ->
+    c  -[ tm ]->* c''
+
+  where "c -[ tm ]->* c'" := (evstep tm c c').
+
+#[export] Hint Constructors evstep : core.
+
+
+Reserved Notation "c -[ tm ]->+ c'" (at level 40).
+
+Inductive progress (tm : TM) : DH_config -> DH_config -> Prop :=
+  | progress_base c c' :
+    c -[ tm ]->  c' ->
+    c -[ tm ]->+ c'
+  | progress_step c c' c'' :
+    c  -[ tm ]->  c'  ->
+    c' -[ tm ]->+ c'' ->
+    c  -[ tm ]->+ c''
+
+  where "c -[ tm ]->+ c'" := (progress tm c c').
+
+Arguments progress_base {tm c c'}.
+Arguments progress_step {tm c c' c''}.
+
+#[export] Hint Constructors progress : core.
+
+
+Definition halted (tm : TM) (c : DH_config) : Prop :=
+  match c with
+  | (l,m >> r,s,sgn) => tm (s,m) = None
+  end.
+
+Definition halts_in (tm : TM) (c : DH_config) (n : nat) :=
+  exists ch, c -[ tm ]->> n / ch /\ halted tm ch.
+
+Definition halts (tm : TM) (c0 : DH_config) :=
+  exists n, halts_in tm c0 n.
+
+Definition c0 : DH_config := (const s0,const s0,q0,R).
+
+Lemma step_nonhalt : forall tm (P : DH_config -> Prop) c,
+  (forall c, P c -> exists c', P c' /\ c -[ tm ]-> c') ->
+  P c ->
+  ~ halts tm c.
+Proof.
+  introv Hstep H0 Hhalts.
+  destruct Hhalts as [k [c' [H1 H2]]].
+  gen c.
+  induction k; intros c Hc.
+  - destruct (Hstep c Hc) as [c1 [Hc1 Hs]].
+    unfold halted in H2.
+    intros Hc'.
+    inverts Hc'.
+    inverts Hs; congruence.
+  - destruct (Hstep c Hc) as [c1 [Hc1 Hs]].
+    intros HS.
+    inverts HS.
+    unshelve eapply (IHk _ _ H1).
+    inverts Hs; inverts H0; try congruence.
+    + destruct sgn; cbn in H9; congruence.
+    + destruct sgn; cbn in H; congruence.
+Qed.
+
+
+Lemma evstep_trans : forall tm c c' c'',
+  c  -[ tm ]->* c' ->
+  c' -[ tm ]->* c'' ->
+  c  -[ tm ]->* c''.
+Proof.
+  introv H1 H2.
+  induction H1; simpl; eauto.
+Qed.
+
+Lemma multistep_trans : forall tm n m c c' c'',
+  c  -[ tm ]->> n / c' ->
+  c' -[ tm ]->> m / c'' ->
+  c  -[ tm ]->> (n + m) / c''.
+Proof.
+  introv H1 H2.
+  induction H1; simpl; eauto.
+Qed.
+
+Lemma step_deterministic tm c c1 c2:
+  c -[ tm ]-> c1 ->
+  c -[ tm ]-> c2 ->
+  c1 = c2.
+Proof.
+  intros C1 C2.
+  inverts C1.
+  inverts C2.
+  - congruence.
+  - destruct sgn; cbn in H6; congruence.
+  - inverts C2;
+    destruct sgn; cbn in H; congruence.
+Qed.
+
+Lemma no_halted_step : forall tm c,
+  ~ halted tm c ->
+  exists c',
+  c -[ tm ]-> c'.
+Proof.
+  introv Hhalted.
+  destruct c as [[[l [m r]] s] sgn].
+  destruct (tm (s,m)) as [[[m' sgn'] s'] |] eqn:E.
+  - destruct sgn,sgn'; eexists; constructor; apply E.
+  - congruence.
+Qed.
+
+Lemma nonhalt_iff {tm c}:
+  ~halts tm c <->
+  forall n, exists c', c -[ tm ]->> n / c'.
+Proof.
+  split; intros H.
+  - unfold halts,halts_in in H.
+    intros n.
+    induction n.
+    + exists c. constructor.
+    + destruct IHn as [c' IHn].
+      epose proof (no_halted_step tm c' _) as H0.
+      destruct H0 as [c'0 H0].
+      eexists.
+      replace (S n) with (n+1) by lia.
+      eapply multistep_trans; eauto.
+      Unshelve.
+      intros H0.
+      apply H.
+      exists n c'; tauto.
+  - intros H0.
+    destruct H0 as [n [c'' [H0 H1]]].
+    specialize (H (S n)).
+    destruct H as [c' H].
+    gen c c' c''.
+    induction n.
+    + introv C' C'' Hh.
+      inverts C'. inverts C''.
+      inverts H1.
+      unfold halted in Hh.
+      inverts H0; congruence.
+    + intros c c' H2 c'' H3 H4.
+      inverts H2. inverts H3.
+      eapply IHn; eauto.
+      applys_eq H5.
+      eapply step_deterministic; eauto.
+Qed.
+
+
+Lemma step_evstep_progress :
+  forall tm c c' c'',
+  c  -[ tm ]-> c'  ->
+  c' -[ tm ]->* c'' ->
+  c  -[ tm ]->+ c''.
+Proof.
+  introv H1 H2.
+  gen c H1.
+  induction H2.
+  - auto.
+  - intros.
+    eapply progress_step; eauto.
+Qed.
+
+
+Notation DH_cconfig := ((list Sym)*(list Sym)*Q*dir)%type.
+
+Definition DH_cconfig_to_bounded_config(x:DH_cconfig)(l0 r0:side):DH_config :=
+let '(l,r,s,sgn):=x in
+((match sgn with | R => l0 | L => r0 end) <* l, r *> (match sgn with | R => r0 | L => l0 end), s, sgn).
+
+Definition DH_cconfig_to_config(x:DH_cconfig):DH_config :=
+let '(l,r,s,sgn):=x in
+(const s0 <* l, r *> const s0, s, sgn).
+
+Section DH_cconfig_ctx.
+Hypothesis tm:TM.
+
+Definition DH_cconfig_bounded_step(x:DH_cconfig):option DH_cconfig :=
+let '(l,r,s,sgn):=x in
+match r with
+| nil => None
+| m::r0 =>
+  match tm (s,m) with
+  | None => None
+  | Some (m',sgn',s') =>
+    if dir_eqb sgn sgn' then
+      Some (m'::l,r0,s',sgn')
+    else
+      Some (m'::r0,l,s',sgn')
+  end
+end.
+
+Fixpoint DH_config_bounded_steps(x:DH_cconfig)(T:nat):DH_cconfig :=
+match T with
+| O => x
+| S T =>
+  match DH_cconfig_bounded_step x with
+  | None => x
+  | Some x => DH_config_bounded_steps x T
+  end
+end.
+
+Definition DH_cconfig_bounded_progress(x:DH_cconfig)(T:nat):option DH_cconfig :=
+match DH_cconfig_bounded_step x with
+| None => None
+| Some x => Some (DH_config_bounded_steps x T)
+end.
+
+Definition DH_cconfig_step(x:DH_cconfig):option DH_cconfig :=
+let '(l,r,s,sgn):=x in
+match r with
+| nil =>
+  match tm (s,s0) with
+  | None => None
+  | Some (m',sgn',s') =>
+    if dir_eqb sgn sgn' then
+      Some (m'::l,nil,s',sgn')
+    else
+      Some (m'::nil,l,s',sgn')
+  end
+| m::r0 =>
+  match tm (s,m) with
+  | None => None
+  | Some (m',sgn',s') =>
+    if dir_eqb sgn sgn' then
+      Some (m'::l,r0,s',sgn')
+    else
+      Some (m'::r0,l,s',sgn')
+  end
+end.
+
+Definition DH_cconfig_step'(x:DH_cconfig):DH_cconfig+DH_cconfig :=
+match DH_cconfig_step x with
+| None => inr x
+| Some x0 => inl x0
+end.
+
+Definition DH_cconfig_steps(x:DH_cconfig)(T:N):DH_cconfig+DH_cconfig :=
+N_iter_until DH_cconfig_step' (inl x) T.
+
+Definition cc0:DH_cconfig := (nil,nil,q0,R).
+
+Definition clength(x:DH_cconfig) :=
+let '(l,r,s,sgn):=x in
+length l + length r.
+
+Lemma DH_cconfig_bounded_step_spec c c':
+  DH_cconfig_bounded_step c = Some c' ->
+  (clength c = clength c' /\ forall l0 r0,
+  DH_cconfig_to_bounded_config c l0 r0 -[ tm ]-> DH_cconfig_to_bounded_config c' l0 r0).
+Proof.
+  unfold DH_cconfig_bounded_step.
+  destruct c as [[[l r] s] sgn].
+  destruct r as [|m r].
+  1: congruence.
+  destruct (tm (s,m)) as [[[m' sgn'] s']|] eqn:E.
+  2: congruence.
+  intros Hc'.
+  destruct sgn,sgn'; cbn; (split; [|intros l0 r0]; inverts Hc'; cbn; auto).
+  all: lia.
+Qed.
+
+Lemma DH_cconfig_bounded_steps_spec c T:
+  let c' := (DH_config_bounded_steps c T) in
+  clength c = clength c' /\
+  forall l0 r0,
+  DH_cconfig_to_bounded_config c l0 r0 -[ tm ]->* DH_cconfig_to_bounded_config c' l0 r0.
+Proof.
+  gen c.
+  induction T; intros; cbn.
+  - split; constructor.
+  - destruct (DH_cconfig_bounded_step c) eqn:E.
+    2: split; constructor.
+    split.
+    + destruct (DH_cconfig_bounded_step_spec _ _ E) as [H _].
+      rewrite H.
+      apply (IHT p).
+    + econstructor.
+      2: apply IHT.
+      apply DH_cconfig_bounded_step_spec,E.
+Qed.
+
+Lemma DH_cconfig_bounded_progress_spec c T:
+  match DH_cconfig_bounded_progress c T with
+  | Some c' =>
+    clength c = clength c' /\
+    forall l0 r0,
+    DH_cconfig_to_bounded_config c l0 r0 -[ tm ]->+ DH_cconfig_to_bounded_config c' l0 r0
+  | None => True
+  end.
+Proof.
+  unfold DH_cconfig_bounded_progress.
+  destruct (DH_cconfig_bounded_step c) eqn:E; trivial.
+  split.
+  + epose proof (DH_cconfig_bounded_steps_spec p T) as [H _].
+    rewrite <-H.
+    eapply DH_cconfig_bounded_step_spec,E.
+  + intros.
+    eapply step_evstep_progress.
+    - eapply DH_cconfig_bounded_step_spec,E.
+    - eapply DH_cconfig_bounded_steps_spec.
+Qed.
+
+Lemma DH_cconfig_step_spec c:
+  match DH_cconfig_step c with
+  | Some c' => DH_cconfig_to_config c -[ tm ]-> DH_cconfig_to_config c'
+  | None => halted tm (DH_cconfig_to_config c)
+  end.
+Proof.
+  unfold DH_cconfig_step.
+  destruct c as [[[l r] s] sgn].
+  destruct r as [|m r].
+  - destruct (tm (s,s0)) as [[[m' sgn'] s']|] eqn:E.
+    2: congruence.
+    destruct sgn,sgn'; cbn.
+    + applys_eq step_through; eauto.
+      rewrite <-const_unfold; reflexivity.
+    + applys_eq step_back; eauto.
+      1: rewrite <-const_unfold; reflexivity.
+      1: reflexivity.
+      apply E.
+    + applys_eq step_back; eauto.
+      1: rewrite <-const_unfold; reflexivity.
+      1: reflexivity.
+      apply E.
+    + applys_eq step_through; eauto.
+      rewrite <-const_unfold; reflexivity.
+  - destruct (tm (s,m)) as [[[m' sgn'] s']|] eqn:E.
+    2: congruence.
+    destruct sgn,sgn'; cbn; auto.
+Qed.
+
+Lemma DH_cconfig_steps_spec c T:
+  match DH_cconfig_steps c T with
+  | inl c' => DH_cconfig_to_config c -[ tm ]->* DH_cconfig_to_config c'
+  | inr c' => halted tm (DH_cconfig_to_config c')
+  end.
+Proof.
+  apply N_iter_until_spec.
+  2: constructor.
+  intros.
+  unfold DH_cconfig_step'.
+  pose proof (DH_cconfig_step_spec x0).
+  destruct (DH_cconfig_step x0).
+  - eapply evstep_trans; eauto.
+  - auto.
+Qed.
+
+End DH_cconfig_ctx.
+
+Lemma progress_nonhalt : forall tm (P : DH_config -> Prop) c,
+  (forall c, P c -> exists c', P c' /\ c -[ tm ]->+ c') ->
+  P c ->
+  ~ halts tm c.
+Proof.
+  introv Hstep H0.
+  eapply step_nonhalt with (P:=fun c => P c \/ exists c', P c' /\ c -[ tm ]->+ c').
+  2: tauto.
+  intros c1 [H|H].
+  1: destruct (Hstep c1 H) as [c' [H1 H2]].
+  2: destruct H as [c' [H1 H2]].
+  all: destruct H2;
+    [ exists c'; tauto
+    | exists c';
+      split; try tauto;
+      right;
+      exists c''; tauto ].
+Qed.
+
+Lemma step_nonhalted tm c1 c2:
+  c1 -[ tm ]-> c2 ->
+  ~ halted tm c1.
+Proof.
+  unfold halted.
+  intros H H0.
+  inverts H; congruence.
+Qed.
+
+Lemma multistep_nonhalt tm n c1 c2:
+  ~halts tm c2 ->
+  multistep tm n c1 c2 ->
+  ~halts tm c1.
+Proof.
+  gen c1 c2.
+  induction n; introv Hn Hm.
+  - inverts Hm. apply Hn.
+  - inverts Hm.
+    epose proof (IHn c' c2 Hn H1) as Hh.
+    intros [n0 [c3 [H2 H3]]].
+    apply Hh.
+    destruct n0 as [|n0].
+    + inverts H2.
+      destruct (step_nonhalted _ _ _ H0 H3).
+    + inverts H2.
+      assert (c'=c'0) by (eapply step_deterministic; eauto); subst c'0.
+      exists n0 c3; tauto.
+Qed.
+
+Lemma evstep_multistep {tm c1 c2}:
+  evstep tm c1 c2 ->
+  exists n, multistep tm n c1 c2.
+Proof.
+  intros.
+  induction H.
+  - eauto.
+  - destruct IHevstep as [n IH].
+    eauto.
+Qed.
+
+Lemma evstep_nonhalt {tm c1 c2}:
+  ~halts tm c2 ->
+  evstep tm c1 c2 ->
+  ~halts tm c1.
+Proof.
+  intros Hh He.
+  destruct (evstep_multistep He) as [n Hm].
+  eapply multistep_nonhalt; eauto.
+Qed.
+
+Definition step_c(tm:TM)(c:DH_config):option (DH_config) :=
+let '(l,m >> r,s,sgn):=c in
+match tm (s,m) with
+| None => None
+| Some (m',sgn',s') =>
+  if dir_eqb sgn sgn' then
+    Some (m' >> l,r,s',sgn')
+  else
+    Some (m' >> r,l,s',sgn')
+end.
+
+Fixpoint multistep_c(tm:TM)(n:nat)(c:DH_config) :=
+match n with
+| O => Some c
+| S n =>
+  match step_c tm c with
+  | Some c =>multistep_c tm n c
+  | None => None
+  end
+end.
+
+Definition halts_in' tm c n :=
+exists ch, multistep_c tm n c = Some ch /\ halted tm ch.
+
+Definition halts' tm c :=
+exists n, halts_in' tm c n.
+
+Lemma step_c_spec tm c c':
+  step_c tm c = Some c' <->
+  c -[ tm ]-> c'.
+Proof.
+  split; intros H.
+  - destruct c as [[[l [m r]] s] sgn].
+    cbn in H.
+    destruct (tm (s,m)) as [[[m' sgn'] s']|] eqn:E.
+    2: congruence.
+    destruct sgn,sgn'; inverts H; constructor; auto.
+  - inverts H; cbn; rewrite H0; destruct sgn; reflexivity.
+Qed.
+
+Lemma multistep_c_spec tm n c c':
+  multistep_c tm n c = Some c' <->
+  c -[ tm ]->> n / c'.
+Proof.
+  gen c c'.
+  induction n; intros.
+  - split; intros H; inverts H; constructor.
+  - split; intros H.
+    + cbn in H.
+      destruct (step_c tm c) eqn:E; try congruence.
+      rewrite step_c_spec in E.
+      rewrite IHn in H.
+      eauto.
+    + inverts H. cbn.
+      rewrite <-step_c_spec in H1.
+      rewrite H1,IHn.
+      assumption.
+Qed.
+
+Lemma halts_in_halts_in' {tm c n}:
+  halts_in tm c n <-> halts_in' tm c n.
+Proof.
+  unfold halts_in,halts_in'.
+  split; intros [ch [H H0]]; exists ch; (split;[|tauto]).
+  - rewrite multistep_c_spec.
+    apply H.
+  - rewrite <-multistep_c_spec.
+    apply H.
+Qed.
+
+Lemma halts_halts' {tm c}:
+  halts tm c <-> halts' tm c.
+Proof.
+  unfold halts,halts'.
+  split; intros [n H]; exists n.
+  - rewrite <-halts_in_halts_in'.
+    apply H.
+  - rewrite halts_in_halts_in'.
+    apply H.
+Qed.
+
+End DHTM.
+
+
