verify/Eqb.v
@@ -1,0 +1,116 @@
+Require Import List.
+Require Import ZArith.
+From BusyCoq Require Import LibTactics.
+
+Notation "x || y" := (if x then true else y) : bool_scope.
+Notation "x && y" := (if x then y else false) : bool_scope.
+Open Scope bool.
+
+Lemma or_false_iff (a b:bool):
+  (a || b) = false <->
+  a = false /\ b = false.
+Proof.
+  destruct a,b; tauto.
+Qed.
+
+Lemma and_true_iff (a b:bool):
+  (a && b) = true <->
+  a = true /\ b = true.
+Proof.
+  destruct a,b; tauto.
+Qed.
+
+Definition if_Some{A B}(a:option A)(b:A->option B) :=
+match a with
+| Some a0 => b a0
+| None => None
+end.
+
+Notation "a &&& b" := (if_Some a b) (at level 40, left associativity).
+
+Ltac solve_Bool_reflect :=
+  try (constructor; congruence).
+
+Fixpoint list_eqb{T}(T_eqb:T->T->bool)(a b:list T):bool :=
+match a,b with
+| a0::a1,b0::b1 => (T_eqb a0 b0) && (list_eqb T_eqb a1 b1)
+| nil,nil => true
+| _,_ => false
+end.
+
+Lemma list_eqb_spec {T} T_eqb (a b:list T):
+  (forall a0 b0, Bool.reflect (a0=b0) (T_eqb a0 b0)) ->
+  Bool.reflect (a=b) (list_eqb T_eqb a b).
+Proof.
+  intro H.
+  gen b.
+  induction a as [|a0 a1]; intros b; destruct b as [|b0 b1]; cbn.
+  all: solve_Bool_reflect.
+  destruct (H a0 b0),(IHa1 b1); solve_Bool_reflect.
+Qed.
+
+Definition prod_eqb{A B}(A_eqb:A->A->bool)(B_eqb:B->B->bool)(a b:A*B):bool :=
+match a,b with
+| (a0,a1),(b0,b1) =>
+  A_eqb a0 b0 && B_eqb a1 b1
+end.
+
+Lemma prod_eqb_spec{A B} A_eqb B_eqb (a b:A*B):
+  (forall a0 b0, Bool.reflect (a0=b0) (A_eqb a0 b0)) ->
+  (forall a0 b0, Bool.reflect (a0=b0) (B_eqb a0 b0)) ->
+  Bool.reflect (a=b) (prod_eqb A_eqb B_eqb a b).
+Proof.
+  intros Ha Hb.
+  destruct a as [a0 a1].
+  destruct b as [b0 b1]; cbn.
+  destruct (Ha a0 b0),(Hb a1 b1); solve_Bool_reflect.
+Qed.
+
+Fixpoint Pos_iter_until{S S'}(f:S->S+S')(x:S+S')(T:positive):S+S' :=
+match x with
+| inl s =>
+  match T with
+  | xH => f s
+  | xO T0 => Pos_iter_until f (Pos_iter_until f x T0) T0
+  | xI T0 => Pos_iter_until f (Pos_iter_until f (f s) T0) T0
+  end
+| _ => x
+end.
+
+Definition N_iter_until{S S'}(f:S->S+S')(x:S+S')(T:N):S+S' :=
+match T with
+| N0 => x
+| Npos T0 => Pos_iter_until f x T0
+end.
+
+Lemma N_iter_until_spec{S S'}{f:S->S+S'}{x:S+S'}{T:N}(P:S->Prop)(P':S'->Prop):
+(forall x0:S, P x0 ->
+match f x0 with
+| inl x1 => P x1
+| inr x1 => P' x1
+end) ->
+(match x with
+| inl x1 => P x1
+| inr x1 => P' x1
+end) ->
+match N_iter_until f x T with
+| inl x1 => P x1
+| inr x1 => P' x1
+end.
+Proof.
+  intros H.
+  destruct T as [|T].
+  1: cbn; tauto.
+  cbn.
+  gen x.
+  induction T; intros x Hx; cbn.
+  - destruct x.
+    + apply IHT,IHT,H,Hx.
+    + apply Hx.
+  - destruct x.
+    + apply IHT,IHT,Hx.
+    + apply Hx.
+  - destruct x.
+    + apply H,Hx.
+    + apply Hx.
+Qed.
